@prefix rdf: <http://www.w3.org/1999/02/22-rdf-syntax-ns#>.
@prefix rdfs: <http://www.w3.org/2000/01/rdf-schema#>.
@prefix owl: <http://www.w3.org/2002/07/owl#>.
@prefix xsd: <http://www.w3.org/2001/XMLSchema#>.
@prefix skos: <http://www.w3.org/2004/02/skos/core#>.
@prefix dct: <http://purl.org/dc/terms/>.
@prefix foaf: <http://xmlns.com/foaf/0.1/>.
@prefix cidoc: <http://www.cidoc-crm.org/cidoc-crm/>.
@prefix frbroo: <http://iflastandards.info/ns/fr/frbr/frbroo/>.
@prefix event: <http://www.knora.org/ontology/0047/event#>.
@prefix human: <http://www.knora.org/ontology/0048/human#>.
@prefix text: <http://www.knora.org/ontology/0059/text#>.
@prefix infocar: <http://www.knora.org/ontology/004C/information-carrier#>.
@prefix publish: <http://www.knora.org/ontology/0056/publishing#>.
@prefix knora-base: <http://www.knora.org/ontology/knora-base#>.

@base <http://www.knora.org/ontology/0044/concept>.
@prefix concept: <http://www.knora.org/ontology/0044/concept#>.

<http://www.knora.org/ontology/0044/concept>
	a owl:Ontology;
	dct:title "An ontology about concept"@en;
	dct:description """Formal description of concept, its general subclasses, related classes and properties."""@en;
	dct:creator "Hans Cools, MD, knowledge engineer, ontologist, software developer, NIE-INE, Basel University, Switzerland"@en;
	dct:publisher "Basel University, Switzerland"@en;

	knora-base:attachedToProject <http://rdfh.ch/projects/0044>.

#
# CLASSES
#

concept:Concept
	a owl:Class;
	rdfs:label "concept"@en, "Konzept"@de;
	rdfs:comment """Abstract idea created by a person, as product of mental activity."""@en;
	rdfs:subClassOf human:Creation, frbroo:F6_Concept. # rdfs:subClassOf cidoc:E28_Conceptual_Object

concept:Fiction
	a owl:Class;
	rdfs:label "fiction"@en, "Fiktion"@de;
	rdfs:comment """Concept derived from imagination."""@en;
	rdfs:subClassOf concept:Concept.

concept:Nonfiction
	a owl:Class;
	rdfs:label "nonfiction"@en, "sachliche Expression"@de;
	rdfs:comment """Concept based on fact."""@en;
	rdfs:subClassOf concept:Concept.

concept:Commonplace # related: truism, clichÃ©
	a owl:Class;
	rdfs:label "commonplace"@en, "Gemeinplatz"@de, "lieu commun"@fr;
	rdfs:comment """Concept generally known, not needing any further explanation, e.g. "Romeo and Julia"."""@en;
	rdfs:subClassOf concept:Concept.

concept:SymbolicConcept
	a owl:Class;
	rdfs:label "symbolic concept"@en, "symbolisches Konzept"@de;
	rdfs:comment """Concept represented by one or more symbols."""@en; #*
	rdfs:subClassOf concept:Concept, cidoc:E90_Symbolic_Object, [
		a owl:Restriction; owl:onProperty concept:isPartOf; owl:minCardinality "0"^^xsd:nonNegativeInteger], [
		a owl:Restriction; owl:onProperty concept:isPartOfValue; owl:minCardinality "0"^^xsd:nonNegativeInteger].

concept:PropositionalConcept
	a owl:Class;
	rdfs:label "propositional concept"@en, "propositionales Konzept"@de;
	rdfs:comment """Concept represented by a statement bearing a truth value, e.g. a judgement or opinion."""@en; #*
	skos:note """Different from a linguisitc proposition."""@en;
	rdfs:subClassOf concept:Concept, cidoc:E89_Propositional_Object.

concept:ThoughtBody #* related to belief system related to school of thought related to theory
	a owl:Class;
	rdfs:label "body of thought"@en, "Gedankengut"@de;
	rdfs:comment """Coherent group of propositional concepts."""@en; #*
	rdfs:subClassOf concept:PropositionalConcept.

concept:Work
	a owl:Class;
	rdfs:label "work"@en, "Werk"@de;
	rdfs:comment """Intellectual product as concept."""@en; #*
	rdfs:subClassOf concept:PropositionalConcept, frbroo:F1_Work, [
		a owl:Restriction; owl:onProperty text:hasTitle; owl:minCardinality "0"^^xsd:nonNegativeInteger], [
		a owl:Restriction; owl:onProperty concept:isExpressedIn; owl:minCardinality "0"^^xsd:nonNegativeInteger], [
		a owl:Restriction; owl:onProperty concept:isExpressedInValue; owl:minCardinality "0"^^xsd:nonNegativeInteger].

concept:IndividualWork
	a owl:Class;
	rdfs:label "individual work"@en, "individuelles Werk"@de;
	rdfs:comment """Work as a complete whole realised in one self-contained expression."""@en;
	rdfs:subClassOf concept:Work, frbroo:F14_Individual_Work.

concept:Information
	a owl:Class;
	rdfs:label "information"@en, "Information"@de;
	rdfs:comment """Symbolic propositional concept resolving uncertainty."""@en;
	rdfs:subClassOf concept:PropositionalConcept, concept:SymbolicConcept, cidoc:E73_Information_Object, [
		a owl:Restriction; owl:onProperty infocar:isOnCarrier; owl:minCardinality "0"^^xsd:nonNegativeInteger], [
		a owl:Restriction; owl:onProperty infocar:isOnCarrierValue; owl:minCardinality "0"^^xsd:nonNegativeInteger]. #, [
#		a owl:Restriction; owl:onProperty concept:hasContent; owl:minCardinality "0"^^xsd:nonNegativeInteger].

concept:Set
	a owl:Class;
	rdfs:label "set"@en, "Sammlung"@de;
	rdfs:comment """Set of expressions."""@en;
	rdfs:subClassOf concept:Information.

concept:Cycle
	a owl:Class;
	rdfs:label "cycle"@en, "Zyklus"@de;
	rdfs:comment """Set of expressions belonging together, usually created around a certain theme, and intended to be experienced in a certain sequence."""@en;
	rdfs:subClassOf concept:Set.

concept:Procedure #* -> physical procedure SCO cidoc:E29_Design_or_Procedure
	a owl:Class;
	rdfs:label "procedure"@en, "Vorgehen"@de;
	rdfs:comment """Plan to perform an action in one or more steps, in a certain manner to obtain a certain output under certain circumstances."""@en;
	rdfs:subClassOf concept:Information, cidoc:E29_Design_or_Procedure.

concept:ThoughtMethod #* part/SC of philosophy ?
	a owl:Class;
	rdfs:label "thought method"@en, "Methode des Denkens"@de;
	rdfs:comment """Analysis of facts to form a judgment."""@en;
	rdfs:subClassOf concept:Information.

#concept:CriticalThoughtMethod
#	a owl:Class;
#	rdfs:label "critical thought method"@en, "Methode des kritischen Denkens"@de;
#	rdfs:comment """Objective analysis of facts to form a judgment."""@en;
#	rdfs:subClassOf concept:ThoughtMethod.

concept:Expression
	a owl:Class;
	rdfs:label "expression"@en, "Expression"@de;
	rdfs:comment """Identifiable immaterial symbolic realisation of an individual work, e.g. a text, story, poem, play, musical, song, joke, choreographic notation, movement pattern, sound pattern, image, multimedia object, or any combination of them, having an objectively recognisable structure."""@en;
	rdfs:subClassOf concept:Information, frbroo:F22_Self-Contained_Expression, [
		a owl:Restriction; owl:onProperty text:hasTitle; owl:minCardinality "0"^^xsd:nonNegativeInteger], [
		a owl:Restriction; owl:onProperty infocar:isOnCarrier; owl:minCardinality "0"^^xsd:nonNegativeInteger], [
		a owl:Restriction; owl:onProperty infocar:isOnCarrierValue; owl:minCardinality "0"^^xsd:nonNegativeInteger], [
		a owl:Restriction; owl:onProperty infocar:isOnPage; owl:minCardinality "0"^^xsd:nonNegativeInteger], [
		a owl:Restriction; owl:onProperty infocar:isOnPageValue; owl:minCardinality "0"^^xsd:nonNegativeInteger], [
		a owl:Restriction; owl:onProperty infocar:hasPageNumberDescription; owl:minCardinality "0"^^xsd:nonNegativeInteger], [
		a owl:Restriction; owl:onProperty concept:hasContentSubject; owl:minCardinality "0"^^xsd:nonNegativeInteger], [
		a owl:Restriction; owl:onProperty concept:hasContentSubjectValue; owl:minCardinality "0"^^xsd:nonNegativeInteger], [
		a owl:Restriction; owl:onProperty concept:isPartOfCycle; owl:minCardinality "0"^^xsd:nonNegativeInteger], [
		a owl:Restriction; owl:onProperty concept:isPartOfCycleValue; owl:minCardinality "0"^^xsd:nonNegativeInteger], [
		a owl:Restriction; owl:onProperty publish:hasPublishingState; owl:minCardinality "0"^^xsd:nonNegativeInteger], [
		a owl:Restriction; owl:onProperty publish:hasPublishingStateValue; owl:minCardinality "0"^^xsd:nonNegativeInteger], [
		a owl:Restriction; owl:onProperty publish:hasPublication; owl:minCardinality "0"^^xsd:nonNegativeInteger], [
		a owl:Restriction; owl:onProperty publish:hasPublicationValue; owl:minCardinality "0"^^xsd:nonNegativeInteger], [
		a owl:Restriction; owl:onProperty publish:hasPublicationNumber; owl:minCardinality "0"^^xsd:nonNegativeInteger], [
		a owl:Restriction; owl:onProperty publish:hasLastPublication; owl:minCardinality "0"^^xsd:nonNegativeInteger], [
		a owl:Restriction; owl:onProperty publish:hasLastPublicationValue; owl:minCardinality "0"^^xsd:nonNegativeInteger], [
		a owl:Restriction; owl:onProperty publish:hasLastAuthorizedPublication; owl:minCardinality "0"^^xsd:nonNegativeInteger], [
		a owl:Restriction; owl:onProperty publish:hasLastAuthorizedPublicationValue; owl:minCardinality "0"^^xsd:nonNegativeInteger], [
		a owl:Restriction; owl:onProperty publish:hasUnauthorizedPublication; owl:minCardinality "0"^^xsd:nonNegativeInteger], [
		a owl:Restriction; owl:onProperty publish:hasUnauthorizedPublicationValue; owl:minCardinality "0"^^xsd:nonNegativeInteger], [
		a owl:Restriction; owl:onProperty publish:hasUnauthorizedRepublication; owl:minCardinality "0"^^xsd:nonNegativeInteger], [
		a owl:Restriction; owl:onProperty publish:hasUnauthorizedRepublicationValue; owl:minCardinality "0"^^xsd:nonNegativeInteger], [
		a owl:Restriction; owl:onProperty publish:isPublishedOnline; owl:minCardinality "0"^^xsd:nonNegativeInteger], [
		a owl:Restriction; owl:onProperty publish:isPublishedOnlineValue; owl:minCardinality "0"^^xsd:nonNegativeInteger], [
		a owl:Restriction; owl:onProperty publish:hasPolyAuthorPublication; owl:minCardinality "0"^^xsd:nonNegativeInteger], [
		a owl:Restriction; owl:onProperty publish:hasPolyAuthorPublicationValue; owl:minCardinality "0"^^xsd:nonNegativeInteger], [
		a owl:Restriction; owl:onProperty publish:hasNachlassPublication; owl:minCardinality "0"^^xsd:nonNegativeInteger], [
		a owl:Restriction; owl:onProperty publish:hasNachlassPublicationValue; owl:minCardinality "0"^^xsd:nonNegativeInteger], [
		a owl:Restriction; owl:onProperty publish:hasNachlassPublicationDescription; owl:minCardinality "0"^^xsd:nonNegativeInteger].

# publish:hasMonoAuthorPublication

# to do: concept:PolyAuthorExpression

# public - private

# concept:Religion

#
# PROPERTIES
#

concept:isPartOf
	a owl:ObjectProperty; #, owl:TransitiveProperty;
	rdfs:label "is part of"@en, "ist Teil von"@de;
	rdfs:comment "Relating a symbolic concept to another one it is part of."@en;
	rdfs:domain concept:SymbolicConcept;
	rdfs:range concept:SymbolicConcept;
	rdfs:subPropertyOf cidoc:P106i_forms_part_of, knora-base:hasLinkTo;
	knora-base:subjectClassConstraint concept:SymbolicConcept;
	knora-base:objectClassConstraint concept:SymbolicConcept.

concept:isPartOfValue
	a owl:ObjectProperty;
	rdfs:label "is part of - statement"@en, "ist Teil von - Festlegung"@de;
	rdfs:comment "Relating something to a reification statement of the relation between that something and something else it is part of."@en;
	rdfs:subPropertyOf knora-base:hasLinkToValue;
	knora-base:subjectClassConstraint concept:SymbolicConcept;
	knora-base:objectClassConstraint knora-base:LinkValue.

concept:isExpressedIn
	a owl:ObjectProperty;
	rdfs:label "is expressed in"@en, "ist ausgedruckt in"@de;
	rdfs:comment "Relating a work to an expression thereof."@en;
	rdfs:domain concept:Work;
	rdfs:range concept:Expression;
	rdfs:subPropertyOf frbroo:R9_is_realised_in, knora-base:hasLinkTo;
	knora-base:subjectClassConstraint concept:Work;
	knora-base:objectClassConstraint concept:Expression.

concept:isExpressedInValue
	a owl:ObjectProperty;
	rdfs:label "is expressed in - statement"@en, "ist ausgedruckt in - Festlegung"@de;
	rdfs:comment "Relating a work to a reification statement of the relation between the work and an expression thereof."@en;
	rdfs:subPropertyOf knora-base:hasLinkToValue;
	knora-base:subjectClassConstraint concept:Work;
	knora-base:objectClassConstraint knora-base:LinkValue.

#concept:hasContent
#	a owl:ObjectProperty;
#	rdfs:label "has content"@en, "hat Inhalt"@de;
#	rdfs:comment """Relating information to its content (as object)."""@en;
#	rdfs:subPropertyOf knora-base:hasValue;
#	knora-base:subjectClassConstraint concept:Information;
#	knora-base:objectClassConstraint knora-base:Value. # BUT not allowed in Knora


# frbroo:R3_is_realised_in: more general: frbroo:F1_Work - frbroo:F22_Self-Contained_Expression

concept:hasContentSubject
	a owl:ObjectProperty;
	rdfs:label "has content subject"@en, "hat inhaltliches Thema"@de;
	rdfs:comment """Relating an expression to a content subject thereof."""@en;
	rdfs:domain concept:Expression;
	rdfs:range rdfs:Resource;
	rdfs:subPropertyOf knora-base:hasLinkTo;
	knora-base:subjectClassConstraint concept:Expression;
	knora-base:objectClassConstraint knora-base:Resource.

concept:hasContentSubjectValue
	a owl:ObjectProperty;
	rdfs:label "has content subject - statement"@en, "hat inhaltliches Thema - Festlegung"@de;
	rdfs:comment """Relating an expression to a reification statement of the relation between the expression and a content subject thereof."""@en;
	rdfs:subPropertyOf knora-base:hasLinkToValue;
	knora-base:subjectClassConstraint concept:Expression;
	knora-base:objectClassConstraint knora-base:LinkValue.

concept:isPartOfCycle
	a owl:ObjectProperty;
	rdfs:label "is part of cycle"@en, "ist Teil eines Zyklus"@de;
	rdfs:comment """Relating an expression to a cycle it is part of."""@en;
	rdfs:domain concept:Expression;
	rdfs:range concept:Cycle;
	rdfs:subPropertyOf concept:isPartOf;
	knora-base:subjectClassConstraint concept:Expression;
	knora-base:objectClassConstraint concept:Cycle.

concept:isPartOfCycleValue
	a owl:ObjectProperty;
	rdfs:label "is part of cycle - statement"@en, "ist Teil eines Zyklus - Festlegung"@de;
	rdfs:comment """Relating an expression to a reification statement of the relation between the expression and a cycle it is part of."""@en;
	rdfs:subPropertyOf concept:isPartOfValue;
	knora-base:subjectClassConstraint concept:Expression;
	knora-base:objectClassConstraint knora-base:LinkValue.

concept:hasDedicatedTo #*
	a owl:ObjectProperty;
	rdfs:label "has dedicated to"@en, "hat gewidmet"@de;
	rdfs:comment """Relating a person to another person to whom the former has dedicated something."""@en;
	rdfs:domain human:Person;
	rdfs:range human:Person;
	rdfs:subPropertyOf knora-base:hasLinkTo;
	knora-base:subjectClassConstraint human:Person;
	knora-base:objectClassConstraint human:Person.

concept:hasDedicatedToValue
	a owl:ObjectProperty;
	rdfs:label "is part of cycle - statement"@en, "ist Teil eines Zyklus - Festlegung"@de;
	rdfs:comment """Relating a person to a reification statement of the relation between the person and another person to whom the former has dedicated something."""@en;
	rdfs:subPropertyOf knora-base:hasLinkToValue;
	knora-base:subjectClassConstraint human:Person;
	knora-base:objectClassConstraint knora-base:LinkValue.