@prefix rdfs: <http://www.w3.org/2000/01/rdf-schema#>.
@prefix owl: <http://www.w3.org/2002/07/owl#>.
@prefix xsd: <http://www.w3.org/2001/XMLSchema#>.
@prefix skos: <http://www.w3.org/2004/02/skos/core#>.
@prefix dct: <http://purl.org/dc/terms/>.
@prefix foaf: <http://xmlns.com/foaf/0.1/>.
@prefix cidoc: <http://www.cidoc-crm.org/cidoc-crm/>.
@prefix frbroo: <http://iflastandards.info/ns/fr/frbr/frbroo/>.
@prefix physical: <http://www.knora.org/ontology/0055/physical-resource#>.
@prefix event: <http://www.knora.org/ontology/0047/event#>.
@prefix human: <http://www.knora.org/ontology/0048/human#>.
@prefix concept: <http://www.knora.org/ontology/0044/concept#>.
@prefix text: <http://www.knora.org/ontology/0059/text#>.
@prefix device: <http://www.knora.org/ontology/0045/device#>.
@prefix knora-base: <http://www.knora.org/ontology/knora-base#>.
@prefix salsah-gui: <http://www.knora.org/ontology/salsah-gui#>.

@base <http://www.knora.org/ontology/004C/information-carrier>.
@prefix infocar: <http://www.knora.org/ontology/004C/information-carrier#>.

<http://www.knora.org/ontology/004C/information-carrier>
	a owl:Ontology;
	dct:title "An ontology about information carrier"@en;
	dct:description """Formal description of information carrier in broadest sense, general subclasses, related classes, and properties."""@en;
	dct:creator "Hans Cools, MD, knowledge engineer, ontologist, software developer, NIE-INE, Basel University, Switzerland"@en;
	dct:publisher "Basel University, Switzerland"@en;

	knora-base:attachedToProject <http://rdfh.ch/projects/004C>.

#
# CLASSES
#

infocar:Carrier
 	a owl:Class;
 	rdfs:label "information carrier"@en,"Informationsträger"@de;
 	rdfs:comment """Carrier of information created by a person."""@en;
	skos:note """Includes both F4_Manifestation_Singleton and F5_Item as declared in FRBROO."""@en;
	rdfs:subClassOf human:PhysicalCreation, cidoc:E84_Information_Carrier, [
		a owl:Restriction; owl:onProperty infocar:carrierHasDescription; owl:minCardinality "0"^^xsd:nonNegativeInteger] #, [
#		a owl:Restriction; owl:onProperty physical:isPartOf; owl:minCardinality "0"^^xsd:nonNegativeInteger], [
#		a owl:Restriction; owl:onProperty physical:isPartOfValue; owl:minCardinality "0"^^xsd:nonNegativeInteger], [
#		a owl:Restriction; owl:onProperty image:hasPhotoRepresentation; owl:minCardinality "0"^^xsd:nonNegativeInteger], [
#		a owl:Restriction; owl:onProperty image:hasPhotoRepresentationValue; owl:minCardinality "0"^^xsd:nonNegativeInteger]
		.

#* infocar:Text OR physical as on carrier

infocar:Leaf
	a owl:Class;
	rdfs:label "leaf"@en, "Blatt"@de;
	rdfs:comment """Sheet of a writable substance, e.g. paper or parchment."""@en;
	rdfs:subClassOf infocar:Carrier, [
		a owl:Restriction; owl:onProperty infocar:isLeafOf; owl:minCardinality "0"^^xsd:nonNegativeInteger], [
		a owl:Restriction; owl:onProperty infocar:isLeafOfValue; owl:minCardinality "0"^^xsd:nonNegativeInteger].

infocar:Page
	a owl:Class;
	rdfs:label "page"@en, "Seite"@de;
	rdfs:comment """One of the 2 surfaces of a leaf, e.g. a manuscript, or of a leaf of a book."""@en;
	rdfs:subClassOf infocar:Carrier, [
		a owl:Restriction; owl:onProperty infocar:isPageOf; owl:minCardinality "0"^^xsd:nonNegativeInteger], [
		a owl:Restriction; owl:onProperty infocar:isPageOfValue; owl:minCardinality "0"^^xsd:nonNegativeInteger], [
		a owl:Restriction; owl:onProperty infocar:isPageOfBook; owl:minCardinality "0"^^xsd:nonNegativeInteger], [
		a owl:Restriction; owl:onProperty infocar:isPageOfBookValue; owl:minCardinality "0"^^xsd:nonNegativeInteger], [
		a owl:Restriction; owl:onProperty infocar:pageHasNumber; owl:minCardinality "0"^^xsd:nonNegativeInteger].

infocar:Book
	a owl:Class;
	rdfs:label "book"@en, "Buch"@de;
	rdfs:comment """Set of leafs, e.g. sheets of paper or parchment, binded together along one side, with a front and back cover."""@en;
	rdfs:subClassOf infocar:Carrier.

infocar:Binding
	a owl:Class;
	rdfs:label "binding"@en, "Einband"@de;
	rdfs:comment """Material holding the leafs and covers of a book together."""@en;
	rdfs:subClassOf infocar:Carrier, [
		a owl:Restriction; owl:onProperty infocar:isBindingOf; owl:minCardinality "0"^^xsd:nonNegativeInteger], [
		a owl:Restriction; owl:onProperty infocar:isBindingOfValue; owl:minCardinality "0"^^xsd:nonNegativeInteger].

infocar:Volume
	a owl:Class;
	rdfs:label "volume"@en, "Band"@de;
	rdfs:comment """One of the books carrying an expression materialized in more than one book."""@en;
	rdfs:subClassOf infocar:Book, [
		a owl:Restriction; owl:onProperty infocar:volumeHasNumber; owl:minCardinality "0"^^xsd:nonNegativeInteger].

infocar:Printing
	a owl:Class;
	rdfs:label "printing"@en, "Drucken"@de;
	rdfs:comment """Action of putting an expression on a carrier, e.g. with ink on paper."""@en;
	rdfs:subClassOf human:Action, frbroo:F32_Carrier_Production_Event.

infocar:Printer
	a owl:Class;
	rdfs:label "printer"@en, "Drucker"@de;
	rdfs:comment """Role of an agent - person or organization - printing an expression."""@en;
	rdfs:subClassOf human:AgentRole.

infocar:Print
	a owl:Class;
	rdfs:label "print"@en, "Druck"@de;
	rdfs:comment """An expression printed on a carrier."""@en;
	rdfs:subClassOf infocar:Carrier, [
		a owl:Restriction; owl:onProperty infocar:isPartOfPrintRun; owl:minCardinality "0"^^xsd:nonNegativeInteger], [
		a owl:Restriction; owl:onProperty infocar:isPartOfPrintRunValue; owl:minCardinality "0"^^xsd:nonNegativeInteger].

infocar:PrintRun
	a owl:Class;
	rdfs:label "print run"@en, "Druckauflage"@de, "Tirage"@fr, "Tiratura"@it;
	rdfs:comment """Collection of prints of the same expression, created at one time."""@en;
	skos:note """When applicable, all the prints have the same ISBN, but a different bar code."""@en;
	rdfs:subClassOf human:PhysicalCreation.

infocar:FirstPrint
	a owl:Class;
	rdfs:label "first print"@en, "Erstdruck"@de;
	rdfs:comment """Earliest print of a tex expression."""@en;
	rdfs:subClassOf infocar:Carrier.

infocar:Archive
	a owl:Class;
	rdfs:label "archive"@en, "Archiv"@de;
	rdfs:comment """Collection of files ordered along a method."""@en;
	rdfs:subClassOf human:PhysicalCreation, cidoc:E78_Collection.

infocar:ArchiveElement
	a owl:Class;
	rdfs:label "archive element"@en, "Archiv-Element"@de;
	rdfs:comment """Element of an archive, which can be a single file or a file group."""@en;
	rdfs:subClassOf infocar:Carrier, [
		a owl:Restriction; owl:onProperty infocar:isPartOfArchive; owl:minCardinality "0"^^xsd:nonNegativeInteger], [
		a owl:Restriction; owl:onProperty infocar:isPartOfArchiveValue; owl:minCardinality "0"^^xsd:nonNegativeInteger], [
		a owl:Restriction; owl:onProperty infocar:hasArchiveSignature; owl:minCardinality "0"^^xsd:nonNegativeInteger].

infocar:Nachlass
	a owl:Class;
	rdfs:label "nachlass"@en, "Nachlass"@de;
	rdfs:comment """Collection of materialized expressions of a person as existing after the person's death."""@en;
	rdfs:subClassOf human:PhysicalCreation, cidoc:E78_Collection.

infocar:NachlassElement
	a owl:Class;
	rdfs:label "nachlass element"@en, "Nachlass-Element"@de;
	rdfs:comment """Element of a nachlass."""@en;
	rdfs:subClassOf infocar:Carrier, [
		a owl:Restriction; owl:onProperty infocar:isPartOfNachlass; owl:minCardinality "0"^^xsd:nonNegativeInteger], [
		a owl:Restriction; owl:onProperty infocar:isPartOfNachlassValue; owl:minCardinality "0"^^xsd:nonNegativeInteger].

infocar:WritingUtensil
	a owl:Class;
	rdfs:label "writing utensil"@en, "Schreibzeug"@de;
	rdfs:comment """Object to write with."""@en;
	rdfs:subClassOf human:PhysicalCreation.

infocar:Pencil
	a owl:Class;
	rdfs:label "pencil"@en, "Bleistift"@de;
	rdfs:comment """Elongated cylindrical(-like) object containing a thin rod of graphite for writing or drawing."""@en;
	rdfs:subClassOf infocar:WritingUtensil.

infocar:Pen
	a owl:Class;
	rdfs:label "pen"@en, "Tintenstift"@de;
	rdfs:comment """Elongated cylindrical(-like) hollow object containing ink for writing or drawing."""@en;
	rdfs:subClassOf infocar:WritingUtensil.

infocar:FountainPen
	a owl:Class;
	rdfs:label "fountain pen"@en, "Füller"@de;
	rdfs:comment """Pen with refillable reservoir for fluid ink for feeding a metal nib."""@en;
	rdfs:subClassOf infocar:Pen.

infocar:Typewriter
	a owl:Class;
	rdfs:label "typewriter"@en, "Schreibmaschine"@de;
	rdfs:comment """Writing device with moving parts for letter printing."""@en; # mechanical or electronic 
	rdfs:subClassOf infocar:WritingUtensil.

infocar:Manuscript
	a owl:Class;
	rdfs:label "manuscript"@en, "Manuskript"@de;
	rdfs:comment """Carrier with a handwritten text."""@en;
	rdfs:subClassOf infocar:Carrier, frbroo:F4_Manifestation_Singleton.

infocar:NoteCarrier
	a owl:Class;
	rdfs:label "note carrier"@en,"Notizträger"@de;
	rdfs:comment """Carrier whereon notes are written, e.g. a first registration of thoughts."""@en;
	rdfs:subClassOf infocar:Carrier, frbroo:F4_Manifestation_Singleton.

infocar:Notebook
	a owl:Class;
	rdfs:label "notebook"@en,"Notizbuch"@de;
	rdfs:comment """Book wherein notes are written."""@en;
	rdfs:subClassOf infocar:Book, infocar:NoteCarrier.

infocar:Typescript
	a owl:Class;
	rdfs:label "typescript"@en, "Typoskript"@de;
	rdfs:comment """Carrier with a typewritten text."""@en;
	rdfs:subClassOf infocar:Carrier, frbroo:F4_Manifestation_Singleton.

infocar:Transcription
	a owl:Class;
	rdfs:label "transcription"@en, "Abschrift"@de;
	rdfs:comment """Carrier with a text copied by any method, e.g. handwriting, typewriting, machine copying, printing, digitizing."""@en;
	rdfs:subClassOf human:Copy, infocar:Carrier, frbroo:F4_Manifestation_Singleton.

 # homonym: transcription: conversion from different manifestation, eg. from spoken or recorded sound to written

infocar:ManuelTranscription
	a owl:Class;
	rdfs:label "manuel transcription"@en, "manuelle Abschrift"@de;
	rdfs:comment """Carrier with a handwritten copy of a text."""@en;
	rdfs:subClassOf infocar:Transcription.

infocar:Diary
	a owl:Class;
	rdfs:label "diary"@en,"Tagebuch"@de;
	rdfs:comment """information carrier with periodically, usually daily, described personal experiences and observations."""@en;
	rdfs:subClassOf infocar:Carrier.

infocar:Sender
	a owl:Class;
	rdfs:label "sender"@en, "Sender"@de;
	rdfs:comment """Role of a person sending information on a a carrier."""@en;
	rdfs:subClassOf human:Role.

infocar:Receiver
	a owl:Class;
	rdfs:label "receiver"@en, "Empfänger"@de;
	rdfs:comment """Role of a person receiving information on a a carrier."""@en;
	rdfs:subClassOf human:Role.

infocar:Letter
	a owl:Class;
	rdfs:label "letter"@en, "Brief"@de;
	rdfs:comment """Written text, e.g. on a leaf, intended to be sent from (a) person(s) or (an) Organization(s) to another one, e.g. through a postal system."""@en;
	rdfs:subClassOf infocar:Carrier, frbroo:F4_Manifestation_Singleton, [
		a owl:Restriction; owl:onProperty infocar:hasSender; owl:minCardinality "0"^^xsd:nonNegativeInteger], [
		a owl:Restriction; owl:onProperty infocar:hasSenderValue; owl:minCardinality "0"^^xsd:nonNegativeInteger], [
		a owl:Restriction; owl:onProperty infocar:hasReceiver; owl:minCardinality "0"^^xsd:nonNegativeInteger], [
		a owl:Restriction; owl:onProperty infocar:hasReceiverValue; owl:minCardinality "0"^^xsd:nonNegativeInteger], [
		a owl:Restriction; owl:onProperty infocar:hasSendingLocation; owl:minCardinality "0"^^xsd:nonNegativeInteger], [
		a owl:Restriction; owl:onProperty infocar:hasSendingLocationValue; owl:minCardinality "0"^^xsd:nonNegativeInteger], [
		a owl:Restriction; owl:onProperty infocar:hasReceivingLocation; owl:minCardinality "0"^^xsd:nonNegativeInteger], [
		a owl:Restriction; owl:onProperty infocar:hasReceivingLocationValue; owl:minCardinality "0"^^xsd:nonNegativeInteger].

infocar:Postcard
	a owl:Class;
	rdfs:label "postcard"@en, "Postkarte"@de;
	rdfs:comment """Card with one side, usually with a printed structure, used for writing a message, an address and applying a postage stamp, to be sent through a postal system."""@en;
	rdfs:subClassOf infocar:Carrier, frbroo:F4_Manifestation_Singleton, [
		a owl:Restriction; owl:onProperty infocar:hasSender; owl:minCardinality "0"^^xsd:nonNegativeInteger], [
		a owl:Restriction; owl:onProperty infocar:hasSenderValue; owl:minCardinality "0"^^xsd:nonNegativeInteger], [
		a owl:Restriction; owl:onProperty infocar:hasReceiver; owl:minCardinality "0"^^xsd:nonNegativeInteger], [
		a owl:Restriction; owl:onProperty infocar:hasReceiverValue; owl:minCardinality "0"^^xsd:nonNegativeInteger], [
		a owl:Restriction; owl:onProperty infocar:hasSendingLocation; owl:minCardinality "0"^^xsd:nonNegativeInteger], [
		a owl:Restriction; owl:onProperty infocar:hasSendingLocationValue; owl:minCardinality "0"^^xsd:nonNegativeInteger], [
		a owl:Restriction; owl:onProperty infocar:hasReceivingLocation; owl:minCardinality "0"^^xsd:nonNegativeInteger], [
		a owl:Restriction; owl:onProperty infocar:hasReceivingLocationValue; owl:minCardinality "0"^^xsd:nonNegativeInteger].

infocar:Convolute
	a owl:Class;
	rdfs:label "convolute"@en, "Konvolut"@de;
	rdfs:comment """information carriers, e.g. of drafts, manuscripts, typoscripts or prints, gathered as one."""@en;
	rdfs:subClassOf human:PhysicalCreation, cidoc:E78_Collection, [
		a owl:Restriction; owl:onProperty infocar:convoluteHasTitle; owl:minCardinality "0"^^xsd:nonNegativeInteger], [
		a owl:Restriction; owl:onProperty infocar:convoluteHasDescription; owl:minCardinality "0"^^xsd:nonNegativeInteger], [
		a owl:Restriction; owl:onProperty infocar:convoluteHasSizeDescription; owl:minCardinality "0"^^xsd:nonNegativeInteger], [
		a owl:Restriction; owl:onProperty infocar:convoluteHasOriginDescription; owl:minCardinality "0"^^xsd:nonNegativeInteger], [
		a owl:Restriction; owl:onProperty infocar:convoluteHasContentRepresentation; owl:minCardinality "0"^^xsd:nonNegativeInteger], [
		a owl:Restriction; owl:onProperty infocar:containsEarlierStagesOf; owl:minCardinality "0"^^xsd:nonNegativeInteger], [
		a owl:Restriction; owl:onProperty infocar:containsEarlierStagesOfValue; owl:minCardinality "0"^^xsd:nonNegativeInteger], [
		a owl:Restriction; owl:onProperty infocar:containsEarlierStagesOfPublication; owl:minCardinality "0"^^xsd:nonNegativeInteger], [
		a owl:Restriction; owl:onProperty infocar:containsEarlierStagesOfPublicationValue; owl:minCardinality "0"^^xsd:nonNegativeInteger], [
		a owl:Restriction; owl:onProperty infocar:containsLaterStagesOf; owl:minCardinality "0"^^xsd:nonNegativeInteger], [
		a owl:Restriction; owl:onProperty infocar:containsLaterStagesOfValue; owl:minCardinality "0"^^xsd:nonNegativeInteger], [
		a owl:Restriction; owl:onProperty infocar:hasCarrierCollectionDescription; owl:minCardinality "0"^^xsd:nonNegativeInteger].

infocar:ElectronicCarrier #* data or information storage device
	a owl:Class;
	rdfs:label "electronic information carrier"@en,"elektronischer Informationsträger"@de;
	rdfs:comment """Electronic machine carrying electronic information."""@en;
	rdfs:subClassOf device:ElectronicMachine, infocar:Carrier.

infocar:ElectronicDocument
	a owl:Class;
	rdfs:label "electronic document"@en,"elektronisches Dokument"@de;
	rdfs:comment """Document stored as electronic information."""@en;
	rdfs:subClassOf knora-base:Resource. # infocar:ElectronicData.

infocar:ElectronicBook
	a owl:Class;
	rdfs:label "electronic book"@en,"elektronisches Buch"@de;
	rdfs:comment """Electronic document with a text structure as in a book."""@en;
	rdfs:subClassOf infocar:ElectronicDocument.

# OR electronic/digital document does not exist without a computer

#
# PROPERTIES
#

infocar:carrierHasDescription
	a owl:ObjectProperty;
	rdfs:label "has description"@en, "hat Beschreibung"@de;
	rdfs:comment """Relating an information carrier to a description (as object) thereof."""@en;
	rdfs:subPropertyOf text:hasDescription;
	knora-base:subjectClassConstraint infocar:Carrier;
	knora-base:objectClassConstraint knora-base:TextValue;
	salsah-gui:guiElement salsah-gui:Richtext.

infocar:isOnCarrier
	a owl:ObjectProperty;
	rdfs:label "is on carrier"@en, "ist auf Träger"@de;
	rdfs:comment "Relating information to a carrier it is on."@en;
	rdfs:subPropertyOf knora-base:hasLinkTo;
	knora-base:subjectClassConstraint concept:Information;
	knora-base:objectClassConstraint infocar:Carrier.

infocar:isOnCarrierValue
	a owl:ObjectProperty;
	rdfs:label "is on carrier - statement"@en, "ist auf Träger - Festlegung"@de;
	rdfs:comment "Relating information to a reification statement of the relation between the information and a carrier it is on."@en;
	rdfs:subPropertyOf knora-base:hasLinkToValue;
	knora-base:subjectClassConstraint concept:Information;
	knora-base:objectClassConstraint knora-base:LinkValue.

infocar:isWrittenWith
	a owl:ObjectProperty;
	rdfs:label "is written with"@en, "ist geschrieben mit"@de;
	rdfs:comment "Relating a text to a utensil it is written with."@en;
	rdfs:subPropertyOf knora-base:hasLinkTo;
	knora-base:subjectClassConstraint text:WrittenText;
	knora-base:objectClassConstraint infocar:WritingUtensil.

infocar:isWrittenWithValue
	a owl:ObjectProperty;
	rdfs:label "is is written with - statement"@en, "ist geschrieben mit - Festlegung"@de;
	rdfs:comment "Relating a text to a reification statement of the relation between the text and a utensil it is written with."@en;
	rdfs:subPropertyOf knora-base:hasLinkToValue;
	knora-base:subjectClassConstraint text:WrittenText;
	knora-base:objectClassConstraint knora-base:LinkValue.

infocar:isOnPage
	a owl:ObjectProperty;
	rdfs:label "is on page"@en, "ist auf Seite"@de;
	rdfs:comment """Relating an expression to a carrier page it is on."""@en;
	rdfs:subPropertyOf infocar:isOnCarrier;
	knora-base:subjectClassConstraint concept:Expression;
	knora-base:objectClassConstraint infocar:Page.

infocar:isOnPageValue
	a owl:ObjectProperty;
	rdfs:label "is on page - statement"@en, "ist auf Seite - Festlegung"@de;
	rdfs:comment """Relating an expression to a reification statement of the relation between the expression and a carrier page it is on."""@en;
	rdfs:subPropertyOf infocar:isOnCarrierValue;
	knora-base:subjectClassConstraint concept:Expression;
	knora-base:objectClassConstraint knora-base:LinkValue.

infocar:hasPageNumberDescription
	a owl:ObjectProperty;
	rdfs:label "has page number description"@en, "hat Seitennummerbeschreibung"@de;
	rdfs:comment """Relating an expression to a description (as object) of the number(s) of and possibly a location on (a) pages it is on; examples of the string of its value: "001-002", "01 recto", "O2 (bottom)"."""@en;
	rdfs:subPropertyOf knora-base:hasValue;
	knora-base:subjectClassConstraint concept:Expression;
	knora-base:objectClassConstraint knora-base:TextValue;
	salsah-gui:guiElement salsah-gui:Richtext.

infocar:isPageOf
	a owl:ObjectProperty;
	rdfs:label "is page of"@en, "ist Seite von"@de;
	rdfs:comment """Relating a page to its leaf, single or in a book."""@en;
	rdfs:subPropertyOf physical:isPartOf;
	knora-base:subjectClassConstraint infocar:Page;
	knora-base:objectClassConstraint infocar:Leaf. # owl:disjointUnionOf (infocar:Leaf infocar:Book) # exclusive OR

infocar:isPageOfValue
	a owl:ObjectProperty;
	rdfs:label "is page of - statement"@en, "ist Seite von - Festlegung"@de;
	rdfs:comment """Relating a page to a reification statement of the relation between the page and its leaf, single or in a book."""@en;
	rdfs:subPropertyOf physical:isPartOfValue;
	knora-base:subjectClassConstraint infocar:Page;
	knora-base:objectClassConstraint knora-base:LinkValue.

infocar:isPageOfBook
	a owl:ObjectProperty;
	rdfs:label "is page of book"@en, "ist Seite eines Buchs"@de;
	rdfs:comment """Relating a page to a book its leaf is part of."""@en;
	rdfs:subPropertyOf physical:isPartOf; # owl:propertyChainAxiom (infocar:isPageOf infocar:isLeafOf)
	knora-base:subjectClassConstraint infocar:Page;
	knora-base:objectClassConstraint infocar:Book.

infocar:isPageOfBookValue
	a owl:ObjectProperty;
	rdfs:label "is page of book - statement"@en, "ist Seite eines Buchs - Festlegung"@de;
	rdfs:comment """Relating a page to a reification statement of the relation between the page and a book its leaf is part of."""@en;
	rdfs:subPropertyOf physical:isPartOfValue;
	knora-base:subjectClassConstraint infocar:Page;
	knora-base:objectClassConstraint knora-base:LinkValue.

infocar:pageHasNumber
	a owl:ObjectProperty;
	rdfs:label "page has number"@en, "Seite hat Nummer"@de;
	rdfs:comment """Relating a page to the number (as object) it has."""@en;
	rdfs:subPropertyOf knora-base:hasValue;
	knora-base:subjectClassConstraint infocar:Page;
	knora-base:objectClassConstraint knora-base:IntValue;  #* -> int
	salsah-gui:guiElement salsah-gui:Richtext.

infocar:isLeafOf
	a owl:ObjectProperty;
	rdfs:label "is leaf of"@en, "ist Blatt von"@de;
	rdfs:comment """Relating a leaf to a book it is part of."""@en;
	rdfs:subPropertyOf physical:isPartOf;
	knora-base:subjectClassConstraint infocar:Leaf;
	knora-base:objectClassConstraint infocar:Book.

infocar:isLeafOfValue
	a owl:ObjectProperty;
	rdfs:label "is leaf of - statement"@en, "ist Blatt von - Festlegung"@de;
	rdfs:comment """Relating a leaf to a reification statement of the relation between the leaf and a book it is part of."""@en;
	rdfs:subPropertyOf physical:isPartOfValue;
	knora-base:subjectClassConstraint infocar:Leaf;
	knora-base:objectClassConstraint knora-base:LinkValue.

infocar:isBindingOf
	a owl:ObjectProperty;
	rdfs:label "is binding of"@en, "ist Einband von"@de;
	rdfs:comment """Relating a binding to a book it is part of."""@en;
	rdfs:subPropertyOf physical:isPartOf;
	knora-base:subjectClassConstraint infocar:Binding;
	knora-base:objectClassConstraint infocar:Book.

infocar:isBindingOfValue
	a owl:ObjectProperty;
	rdfs:label "is binding of - statement"@en, "ist Einband von - Festlegung"@de;
	rdfs:comment """Relating a binding to a reification statement of the relation between the binding and a book it is part of."""@en;
	rdfs:subPropertyOf physical:isPartOfValue;
	knora-base:subjectClassConstraint infocar:Binding;
	knora-base:objectClassConstraint knora-base:LinkValue.

#infocar:hasPage
#	a owl:ObjectProperty;
#	rdfs:label "has page"@en;
#	rdfs:comment """Relating a book to a page thereof."""@en;
#	rdfs:subPropertyOf knora-base:hasLinkTo;
#	knora-base:subjectClassConstraint infocar:Book; # owl:propertyChainAxiom (infocar:hasLeaf x:hasSide)
#	knora-base:objectClassConstraint infocar:Page.

#infocar:hasPageValue
#	a owl:ObjectProperty;
#	rdfs:label "has page - statement"@en;
#	rdfs:comment """Relating a book to a reification statement of the relation between the book and a page thereof."""@en;
#	rdfs:subPropertyOf knora-base:hasLinkToValue;
#	knora-base:subjectClassConstraint infocar:Book;
#	knora-base:objectClassConstraint knora-base:LinkValue.

#infocar:hasPageNumber
#	a owl:ObjectProperty;
#	rdfs:label "has page number"@en;
#	rdfs:comment """Relating an expression to the number (as object) of a page it is on."""@en;
#	rdfs:subPropertyOf knora-base:hasValue;
#	knora-base:subjectClassConstraint concept:Expression; # owl:propertyChainAxiom (infocar:isOnPage x:hasNumber)
#	knora-base:objectClassConstraint knora-base:IntValue.

infocar:volumeHasNumber
	a owl:ObjectProperty;
	rdfs:label "volume has number"@en, "Band hat Nummer"@de;
	rdfs:comment "Relating a volume to its sequence number."@en;
	rdfs:subPropertyOf knora-base:hasValue;
	knora-base:subjectClassConstraint infocar:Volume;
	knora-base:objectClassConstraint knora-base:IntValue.

infocar:isInManuscript
	a owl:ObjectProperty;
	rdfs:label "is in manuscript"@en, "ist in Manuskript"@de;
	rdfs:comment "Relating a handwritten text to the manuscript that carries it."@en;
	rdfs:subPropertyOf infocar:isOnCarrier;
	knora-base:subjectClassConstraint text:HandwrittenText;
	knora-base:objectClassConstraint infocar:Manuscript.

infocar:isInManuscriptValue
	a owl:ObjectProperty;
	rdfs:label "is in manuscript - statement"@en, "ist in Manuskript - Festlegung"@de;
	rdfs:comment "Relating a handwritten text to a reification statement of the relation between the handwritten text and the manuscript that carries it."@en;
	rdfs:subPropertyOf infocar:isOnCarrierValue;
	knora-base:subjectClassConstraint text:HandwrittenText;
	knora-base:objectClassConstraint knora-base:LinkValue.

infocar:isInTypescript
	a owl:ObjectProperty;
	rdfs:label "is in typescript"@en, "ist in Typoskript"@de;
	rdfs:comment "Relating a typewritten text to the typescript that carries it."@en;
	rdfs:subPropertyOf infocar:isOnCarrier;
	knora-base:subjectClassConstraint text:TypewrittenText;
	knora-base:objectClassConstraint infocar:Typescript.

infocar:isInTypescriptValue
	a owl:ObjectProperty;
	rdfs:label "is in typescript - statement"@en, "ist in Typoskript - Festlegung"@de;
	rdfs:comment "Relating a typewritten text to a reification statement of the relation between the typewritten text and the typescript that carries it."@en;
	rdfs:subPropertyOf infocar:isOnCarrierValue;
	knora-base:subjectClassConstraint text:TypewrittenText;
	knora-base:objectClassConstraint knora-base:LinkValue.

infocar:isInDiary
	a owl:ObjectProperty;
	rdfs:label "is in diary"@en, "ist in Tagebuch"@de;
	rdfs:comment """Relating a diary entry to a diary it is in."""@en;
	rdfs:subPropertyOf infocar:isOnCarrier;
	knora-base:subjectClassConstraint text:DiaryEntry;
	knora-base:objectClassConstraint infocar:Diary.

infocar:isInDiaryValue
	a owl:ObjectProperty;
	rdfs:label "is in diary - statement"@en, "ist in Tagebuch - Festlegung"@de;
	rdfs:comment """Relating a diary entry to a reification statement of the relation between the diary entry and a diary it is in."""@en;
	rdfs:subPropertyOf infocar:isOnCarrierValue;
	knora-base:subjectClassConstraint text:DiaryEntry;
	knora-base:objectClassConstraint knora-base:LinkValue.

infocar:hasDiaryEnteringDate
	a owl:ObjectProperty;
	rdfs:label "has diary entering date"@en, "hat Tagebucheintragsdatum"@de;
	rdfs:comment """Relating a diary entry to its date of entering in a diary."""@en;
	rdfs:subPropertyOf human:hasCreationDate;
	knora-base:subjectClassConstraint text:DiaryEntry;
	knora-base:objectClassConstraint knora-base:DateValue;
	salsah-gui:guiElement salsah-gui:Date.

infocar:isInLetter
	a owl:ObjectProperty;
	rdfs:label "is in letter"@en, "ist in Brief"@de;
	rdfs:comment """Relating a letter expression to a letter it is in."""@en;
	rdfs:subPropertyOf infocar:isOnCarrier;
	knora-base:subjectClassConstraint text:LetterExpression;
	knora-base:objectClassConstraint infocar:Letter.

infocar:isInLetterValue
	a owl:ObjectProperty;
	rdfs:label "is in letter - statement"@en, "ist in Brief - Festlegung"@de;
	rdfs:comment """Relating a letter expression to a reification statement of the relation between the letter expression and a letter it is in."""@en;
	rdfs:subPropertyOf infocar:isOnCarrierValue;
	knora-base:subjectClassConstraint text:LetterExpression;
	knora-base:objectClassConstraint knora-base:LinkValue.

infocar:hasSender
	a owl:ObjectProperty;
	rdfs:label "has sender"@en, "hat Absender"@de;
	rdfs:comment """Relating something to a person who sent it."""@en; #* or an Organization -> foaf:Agent
	rdfs:domain knora-base:Resource; #*
#	rdfs:range [rdfs:subClassOf human:Person, [a owl:Restriction; owl:onProperty event:hasRole; owl:someValuesFrom infocar:Sender]];
	rdfs:subPropertyOf knora-base:hasLinkTo;
	knora-base:subjectClassConstraint knora-base:Resource; #*
	knora-base:objectClassConstraint human:Person.

infocar:hasSenderValue
	a owl:ObjectProperty;
	rdfs:label "has sender - statement"@en, "hat Absender - Festlegung"@de;
	rdfs:comment """Relating something to a reification statement of the relation between that something and a person who sent it."""@en;
	rdfs:subPropertyOf knora-base:hasLinkToValue;
	knora-base:subjectClassConstraint knora-base:Resource; #*
	knora-base:objectClassConstraint knora-base:LinkValue.

infocar:hasReceiver
	a owl:ObjectProperty;
	rdfs:label "has receiver"@en, "hat Empfänger"@de;
	rdfs:comment """Relating something to a person who received it."""@en; #* or an Organization -> foaf:Agent
	rdfs:domain knora-base:Resource; #*
#	rdfs:range [rdfs:subClassOf human:Person, [a owl:Restriction; owl:onProperty event:hasRole; owl:someValuesFrom infocar:Receiver]];
	rdfs:subPropertyOf knora-base:hasLinkTo;
	knora-base:subjectClassConstraint knora-base:Resource; #*
	knora-base:objectClassConstraint human:Person.

infocar:hasReceiverValue
	a owl:ObjectProperty;
	rdfs:label "has receiver - statement"@en, "hat Empfänger - Festlegung"@de;
	rdfs:comment """Relating something to a reification statement of the relation between that something and a person who received it."""@en;
	rdfs:subPropertyOf knora-base:hasLinkToValue;
	knora-base:subjectClassConstraint knora-base:Resource; #*
	knora-base:objectClassConstraint knora-base:LinkValue.

infocar:hasSendingLocation
	a owl:ObjectProperty;
	rdfs:label "has sending location"@en, "hat Absendeort"@de;
	rdfs:comment """Relating something to a location it was sent from."""@en;
	rdfs:domain rdfs:Resource;
	rdfs:range physical:Place;
	rdfs:subPropertyOf physical:hasLocation;
	knora-base:subjectClassConstraint knora-base:Resource; #*
	knora-base:objectClassConstraint physical:Place.

infocar:hasSendingLocationValue
	a owl:ObjectProperty;
	rdfs:label "has sending location - statement"@en, "hat Absendeort - Festlegung"@de;
	rdfs:comment """Relating something to a reification statement of the relation between that something and a location it was sent from."""@en;
	rdfs:subPropertyOf physical:hasLocationValue;
	knora-base:subjectClassConstraint knora-base:Resource; #*
	knora-base:objectClassConstraint knora-base:LinkValue.

infocar:hasReceivingLocation
	a owl:ObjectProperty;
	rdfs:label "has receiving location"@en, "hat Empfangort"@de; #*
	rdfs:comment """Relating something to a location it was sent to."""@en;
	rdfs:domain rdfs:Resource;
	rdfs:range physical:Place;
	rdfs:subPropertyOf physical:hasLocation;
	knora-base:subjectClassConstraint knora-base:Resource; #*
	knora-base:objectClassConstraint physical:Place.

infocar:hasReceivingLocationValue
	a owl:ObjectProperty;
	rdfs:label "has receiving location - statement"@en, "hat Empfangort - Festlegung"@de;
	rdfs:comment """Relating something to a reification statement of the relation between that something and a location it was sent to."""@en;
	rdfs:subPropertyOf physical:hasLocationValue;
	knora-base:subjectClassConstraint knora-base:Resource; #*
	knora-base:objectClassConstraint knora-base:LinkValue.

infocar:convoluteHasTitle
	a owl:ObjectProperty;
	rdfs:label "convolute has title"@en, "Konvolut hat Titel"@de;
	rdfs:comment """Relating a convolute to its titel (as object)."""@en;
	rdfs:subPropertyOf text:hasTitle;
	knora-base:subjectClassConstraint infocar:Convolute;
	knora-base:objectClassConstraint knora-base:TextValue;
	salsah-gui:guiElement salsah-gui:Richtext.

infocar:convoluteHasDescription
	a owl:ObjectProperty;
	rdfs:label "convolute has description"@en, "Konvolut hat Beschreibung"@de;
	rdfs:comment """Relating a convolute to a description (as object) thereof."""@en;
	rdfs:subPropertyOf text:hasDescription;
	knora-base:subjectClassConstraint infocar:Convolute;
	knora-base:objectClassConstraint knora-base:TextValue;
	salsah-gui:guiElement salsah-gui:Richtext.

infocar:convoluteHasSizeDescription
	a owl:ObjectProperty;
	rdfs:label "convolute has size description"@en, "Konvolutgrösse hat Beschreibung"@de;
	rdfs:comment """Relating a convolute to a description (as object) of its size."""@en;
	rdfs:subPropertyOf text:hasDescription;
	knora-base:subjectClassConstraint infocar:Convolute;
	knora-base:objectClassConstraint knora-base:TextValue;
	salsah-gui:guiElement salsah-gui:Richtext.

infocar:convoluteHasOriginDescription
	a owl:ObjectProperty;
	rdfs:label "convolute has origin description"@en, "Konvolut hat Herkunftbeschreibung"@de;
	rdfs:comment """Relating a text convolute to a description (as object) of its origin."""@en;
	rdfs:subPropertyOf text:hasDescription;
	knora-base:subjectClassConstraint infocar:Convolute;
	knora-base:objectClassConstraint knora-base:TextValue;
	salsah-gui:guiElement salsah-gui:Richtext.

infocar:convoluteHasContentRepresentation
	a owl:ObjectProperty;
	rdfs:label "convolute has content representation"@en, "Konvolut hat Inhaltrepräsentation"@de;
	rdfs:comment """Relating a convolute to a description (as object) of its content representation."""@en;
	rdfs:subPropertyOf text:hasDescription;
	knora-base:subjectClassConstraint infocar:Convolute;
	knora-base:objectClassConstraint knora-base:TextValue;
	salsah-gui:guiElement salsah-gui:Richtext.

infocar:containsEarlierStagesOf
	a owl:ObjectProperty; # , owl:TransitiveProperty;
	rdfs:label "contains earlier stages of"@en, "enthält frühere Stufen von"@de;
	rdfs:comment """Relating a convolute to another one whose information carriers bear later stages of the texts on the carriers of the former."""@en;
	rdfs:subPropertyOf knora-base:hasLinkTo;
	knora-base:subjectClassConstraint infocar:Convolute;
	knora-base:objectClassConstraint infocar:Convolute.

infocar:containsEarlierStagesOfValue
	a owl:ObjectProperty;
	rdfs:label "contains earlier stages of - statement"@en, "enthält frühere Stufen von - Festlegung"@de;
	rdfs:comment """Relating a convolute to a reification statement of the relation between the convolute and another one whose information carriers bear later stages of the texts on the carriers of the former."""@en;
	rdfs:subPropertyOf knora-base:hasLinkToValue;
	knora-base:subjectClassConstraint infocar:Convolute;
	knora-base:objectClassConstraint knora-base:LinkValue.

infocar:containsEarlierStagesOfPublication
	a owl:ObjectProperty; # , owl:TransitiveProperty;
	rdfs:label "contains earlier stages of publication"@en, "enthält frühere Stufen von Publikation"@de;
	rdfs:comment """Relating a convolute to another one whose information carriers bear later publication stages of the texts on the carriers of the former."""@en;
	rdfs:subPropertyOf infocar:containsEarlierStagesOf;
	knora-base:subjectClassConstraint infocar:Convolute;
	knora-base:objectClassConstraint infocar:Convolute.

infocar:containsEarlierStagesOfPublicationValue
	a owl:ObjectProperty;
	rdfs:label "contains earlier stages of publication - statement"@en, "enthält frühere Stufen von Herausgabe - Festlegung"@de;
	rdfs:comment """Relating a convolute to a reification statement of the relation between the convolute and another one whose information carriers bear later publication stages of the texts on the carriers of the former."""@en;
	rdfs:subPropertyOf infocar:containsEarlierStagesOfValue;
	knora-base:subjectClassConstraint infocar:Convolute;
	knora-base:objectClassConstraint knora-base:LinkValue.

infocar:containsLaterStagesOf
	a owl:ObjectProperty; # , owl:TransitiveProperty;
	rdfs:label "contains later stages of"@en, "enthält spätere Stufen von"@de;
	rdfs:comment """Relating a convolute to another one whose information carriers bear earlier stages of the texts on the carriers of the former."""@en;
	rdfs:subPropertyOf knora-base:hasLinkTo;
	knora-base:subjectClassConstraint infocar:Convolute;
	knora-base:objectClassConstraint infocar:Convolute.

infocar:containsLaterStagesOfValue
	a owl:ObjectProperty;
	rdfs:label "contains later stages of - statement"@en, "enthält spätere Stufen von - Festlegung"@de;
	rdfs:comment """Relating a convolute to a reification statement of the relation between the convolute and another one whose information carriers bear later stages of the texts on the carriers of the former."""@en;
	rdfs:subPropertyOf knora-base:hasLinkToValue;
	knora-base:subjectClassConstraint infocar:Convolute;
	knora-base:objectClassConstraint knora-base:LinkValue.

infocar:hasCarrierCollectionDescription
	a owl:ObjectProperty;
	rdfs:label "has information carrier collection description"@en, "hat Textträgersammlung-Beschreibung"@de;
	rdfs:comment """Relating a convolute to a description (as object) of an information carrier collection it contains."""@en;
	rdfs:subPropertyOf text:hasDescription;
	knora-base:subjectClassConstraint infocar:Convolute;
	knora-base:objectClassConstraint knora-base:TextValue;
	salsah-gui:guiElement salsah-gui:Richtext.

infocar:isPartOfPrintRun
	a owl:ObjectProperty;
	rdfs:label "is part of print run"@en, "ist Teil einer Druckauflage"@de;
	rdfs:comment """Relating a print to the run it is part of."""@en;
	rdfs:subPropertyOf physical:isPartOf;
	knora-base:subjectClassConstraint infocar:Print;
	knora-base:objectClassConstraint infocar:PrintRun.

infocar:isPartOfPrintRunValue
	a owl:ObjectProperty;
	rdfs:label "is part of print run - statement"@en, "ist Teil einer Druckauflage - Festlegung"@de;
	rdfs:comment """Relating a print to a reification statement of the relation between the print and the run it is part of."""@en;
	rdfs:subPropertyOf physical:isPartOfValue;
	knora-base:subjectClassConstraint infocar:Print;
	knora-base:objectClassConstraint knora-base:LinkValue.

infocar:isPartOfArchive
	a owl:ObjectProperty;
	rdfs:label "is part of archive"@en, "ist Teil eines Archivs"@de;
	rdfs:comment """Relating an element of an archive to the archive."""@en;
	rdfs:subPropertyOf physical:isPartOf;
	knora-base:subjectClassConstraint infocar:ArchiveElement;
	knora-base:objectClassConstraint infocar:Archive.

infocar:isPartOfArchiveValue
	a owl:ObjectProperty;
	rdfs:label "is part of archive - statement"@en, "ist Teil eines Archivs - Festlegung"@de;
	rdfs:comment """Relating an element of an archive to a reification statement of the relation between the element and the archive."""@en;
	rdfs:subPropertyOf physical:isPartOfValue;
	knora-base:subjectClassConstraint infocar:ArchiveElement;
	knora-base:objectClassConstraint knora-base:LinkValue.

infocar:hasArchiveSignature
	a owl:ObjectProperty;
	rdfs:label "has archive signature"@en, "hat Archivsignatur"@de;
	rdfs:comment """Relating an element of an archive to its signature (as object) as identifier."""@en;
	rdfs:subPropertyOf text:hasIdentifier;
	knora-base:subjectClassConstraint infocar:ArchiveElement;
	knora-base:objectClassConstraint knora-base:TextValue.

infocar:isPartOfNachlass
	a owl:ObjectProperty;
	rdfs:label "is part of a nachlass"@en, "ist Teil eines Nachlasses"@de;
	rdfs:comment """Relating an element of a nachlass to the nachlass."""@en;
	rdfs:subPropertyOf physical:isPartOf;
	knora-base:subjectClassConstraint infocar:NachlassElement;
	knora-base:objectClassConstraint infocar:Nachlass.

infocar:isPartOfNachlassValue
	a owl:ObjectProperty;
	rdfs:label "is part of a nachlass - statement"@en, "ist Teil eines Nachlasses - Festlegung"@de;
	rdfs:comment """Relating an element of a nachlass to a reification statement of the relation between the element and the nachlass."""@en;
	rdfs:subPropertyOf physical:isPartOfValue;
	knora-base:subjectClassConstraint infocar:NachlassElement;
	knora-base:objectClassConstraint knora-base:LinkValue.