@prefix rdfs: <http://www.w3.org/2000/01/rdf-schema#>.
@prefix owl: <http://www.w3.org/2002/07/owl#>.
@prefix xsd: <http://www.w3.org/2001/XMLSchema#>.
@prefix skos: <http://www.w3.org/2004/02/skos/core#>.
@prefix dct: <http://purl.org/dc/terms/>.
@prefix foaf: <http://xmlns.com/foaf/0.1/>.
@prefix unicore: <http://purl.uniprot.org/core/>.
@prefix cidoc: <http://www.cidoc-crm.org/cidoc-crm/>.
@prefix frbroo: <http://iflastandards.info/ns/fr/frbr/frbroo/>.
@prefix event: <http://www.knora.org/ontology/0047/event#>.
@prefix agent: <http://www.knora.org/ontology/0040/agent#>.
@prefix human: <http://www.knora.org/ontology/0048/human#>.
@prefix concept: <http://www.knora.org/ontology/0044/concept#>.
@prefix text: <http://www.knora.org/ontology/0059/text#>.
@prefix device: <http://www.knora.org/ontology/0045/device#>.
@prefix knora-base: <http://www.knora.org/ontology/knora-base#>.
@prefix salsah-gui: <http://www.knora.org/ontology/salsah-gui#>.

@base <http://www.knora.org/ontology/004F/language>.
@prefix language: <http://www.knora.org/ontology/004F/language#>.

<http://www.knora.org/ontology/004F/language>
	a owl:Ontology;
	dct:title "An ontology about language"@en;
	dct:description """Formal description of language, general subclasses, related classes and properties."""@en;
	dct:creator "Hans Cools, MD, knowledge engineer, ontologist, software developer, NIE-INE, Basel University, Switzerland"@en;
	dct:publisher "Basel University, Switzerland"@en;

	knora-base:attachedToProject <http://rdfh.ch/projects/004F>.

#
# CLASSES
#

language:Language #* to be linked to ability
	a owl:Class;
	rdfs:label "language"@en, "Sprache"@de;
	rdfs:comment """ to express meaning using carriers (e.g. a symbol, sign, word) along rules or grammar model, e.g. syntax for serialization."""@en;
	# Dynamic set of sensory signs, including sounds and gestures, of communication and the semantic, pragmatic, and grammar elements or rules to manipulate them. # dct:LinguisticSystem
	rdfs:subClassOf knora-base:Resource.

language:HumanLanguage
	a owl:Class;
	rdfs:label "human language"@en, "menschliche Sprache"@de;
	rdfs:comment """Language of a human."""@en;
	rdfs:subClassOf language:Language. #*, human:Ability.

language:HumanNaturalLanguage
	a owl:Class;
	rdfs:label "human natural language"@en, "menschliche naturliche Sprache"@de;
	rdfs:comment """Language naturally evolved in humans."""@en;
	skos:note """Excluded is formal language, e.g. computer programming language."""@en;
	rdfs:subClassOf language:HumanLanguage, [
		a owl:Restriction; owl:onProperty language:hasCode; owl:minCardinality "0"^^xsd:nonNegativeInteger].
#	owl:disjointWith language:FormalLanguage.

language:English
	a owl:Class;
	rdfs:label "English"@en, "Englisch"@de;
	rdfs:comment """The language of England, widely used in many varieties throughout the world."""@en;
	rdfs:subClassOf language:HumanNaturalLanguage.

language:HumanNaturalLanguageExpression
	a owl:Class;
	rdfs:label "human natural language expression"@en, "menschliche naturliche sprachliche Äusserung"@de;
	rdfs:comment """Expression in a human natural language, being text in most abstract sense, as writable."""@en;
	skos:note """Different from the FRBROO based concept:Expression."""@en;
	rdfs:subClassOf concept:Information, cidoc:E33_Linguistic_Object, [
		a owl:Restriction; owl:onProperty language:hasContent; owl:minCardinality "0"^^xsd:nonNegativeInteger], [
		a owl:Restriction; owl:onProperty language:expressedInNaturalLanguage; owl:minCardinality "0"^^xsd:nonNegativeInteger], [
		a owl:Restriction; owl:onProperty language:expressedInNaturalLanguageValue; owl:minCardinality "0"^^xsd:nonNegativeInteger], [
		a owl:Restriction; owl:onProperty language:expressedInDialect; owl:minCardinality "0"^^xsd:nonNegativeInteger], [
		a owl:Restriction; owl:onProperty language:expressedInDialectValue; owl:minCardinality "0"^^xsd:nonNegativeInteger], [
		a owl:Restriction; owl:onProperty language:hasTranslator; owl:minCardinality "0"^^xsd:nonNegativeInteger], [
		a owl:Restriction; owl:onProperty language:hasTranslatorValue; owl:minCardinality "0"^^xsd:nonNegativeInteger], [
#		language:hasMachineTranslator
#		language:hasMachineTranslatorValue
		a owl:Restriction; owl:onProperty language:translatedInNaturalLanguage; owl:minCardinality "0"^^xsd:nonNegativeInteger], [
		a owl:Restriction; owl:onProperty language:translatedInNaturalLanguageValue; owl:minCardinality "0"^^xsd:nonNegativeInteger], [
		a owl:Restriction; owl:onProperty language:translatedIn; owl:minCardinality "0"^^xsd:nonNegativeInteger], [
		a owl:Restriction; owl:onProperty language:translatedInValue; owl:minCardinality "0"^^xsd:nonNegativeInteger].

language:Dialect
	a owl:Class;
	rdfs:label "dialect"@en, "Mundart"@de;
	rdfs:comment """Regional variant of a standard language."""@en;
	rdfs:subClassOf language:HumanNaturalLanguage.

language:Translator #*
	a owl:Class;
	rdfs:label "translator"@en, "Übersetzer"@de;
	rdfs:comment """Role of an agent transferring a human natural language expression in another natural language."""@en;
	rdfs:subClassOf agent:Role.

language:PersonTranslator
	a owl:Class;
	rdfs:label "person-translator"@en, "Person-Übersetzer"@de;
	rdfs:comment """Role of a person as translator."""@en;
	rdfs:subClassOf language:Translator, human:Creator.

language:Translation #* OR result of translating with translated text as its object 
	a owl:Class;
	rdfs:label "translation"@en, "Übersetzung"@de;
	rdfs:comment """Human natural language expression transferred in another natural language."""@en;
	rdfs:subClassOf language:HumanNaturalLanguageExpression. #, event:Output.

language:PersonTranslation
	a owl:Class;
	rdfs:label "person's translation"@en, "Übersetzung einer Person"@de;
	rdfs:comment """Translation done by a person."""@en;
	rdfs:subClassOf language:Translation, human:CreationDerivative.

language:MachineTranslation
	a owl:Class;
	rdfs:label "machine translation"@en, "maschinelle Übersetzung"@de;
	rdfs:comment """Translation done by a digital electronic computer using translation software."""@en;
	rdfs:subClassOf language:Translation.

#
# PROPERTIES
#

language:hasCode
	a owl:ObjectProperty;
	rdfs:label "language has code"@en, "Sprache hat Kode"@de;
	rdfs:comment """Relating a language to a code (object) representing that language."""@en;
#	rdfs:domain language:HumanNaturalLanguage;
#	rdfs:range skos:Concept;
	rdfs:subPropertyOf knora-base:hasValue; # skos:exactMatch
	knora-base:subjectClassConstraint language:HumanNaturalLanguage;
	knora-base:objectClassConstraint knora-base:TextValue. 

language:hasContent
	a owl:ObjectProperty;
	rdfs:label "has content"@en, "hat Inhalt"@de;
	rdfs:comment """Relating a human natural language expression to its content (as object)."""@en;
	rdfs:domain language:HumanNaturalLanguageExpression;
	rdfs:range knora-base:TextValue;
	rdfs:subPropertyOf knora-base:hasValue; #* concept:hasContent
	knora-base:subjectClassConstraint language:HumanNaturalLanguageExpression;
	knora-base:objectClassConstraint knora-base:TextValue;
	salsah-gui:guiElement salsah-gui:Richtext.

language:expressedInNaturalLanguage
	a owl:ObjectProperty;
	rdfs:label "expressed in natural language"@en, "geäußert in naturlichen Sprache"@de;
	rdfs:comment """Relating a human expression to a natural language wherein it is expressed."""@en;
	rdfs:domain language:HumanNaturalLanguageExpression;
	rdfs:range language:HumanNaturalLanguage;
	rdfs:subPropertyOf cidoc:P72_has_language, knora-base:hasLinkTo;
	knora-base:subjectClassConstraint language:HumanNaturalLanguageExpression;
	knora-base:objectClassConstraint language:HumanNaturalLanguage.

language:expressedInNaturalLanguageValue
	a owl:ObjectProperty;
	rdfs:label "expressed in natural language - statement"@en, "geäußert in naturlichen Sprache - Festlegung"@de;
	rdfs:comment """Relating a human expression to a reification statement of the relation between the expression and a natural language wherein it is expressed."""@en;
	rdfs:subPropertyOf knora-base:hasLinkToValue;
	knora-base:subjectClassConstraint language:HumanNaturalLanguageExpression;
	knora-base:objectClassConstraint knora-base:LinkValue.

language:expressedInDialect #*
	a owl:ObjectProperty;
	rdfs:label "expressed in dialect"@en, "geäußert in Mundart"@de;
	rdfs:comment """Relating a human expression to a dialect it is expressed in."""@en;
	rdfs:domain language:HumanNaturalLanguageExpression;
	rdfs:range language:Dialect;
	rdfs:subPropertyOf knora-base:hasLinkTo;
	knora-base:subjectClassConstraint language:HumanNaturalLanguageExpression;
	knora-base:objectClassConstraint language:Dialect.

language:expressedInDialectValue
	a owl:ObjectProperty;
	rdfs:label "expressed in dialect - statement"@en, "geäußert in Mundart - Festlegung"@de;
	rdfs:comment "Relating a human expression to a reification statement of the relation between the expression and a dialect it is expressed in."@en;
	rdfs:subPropertyOf knora-base:hasLinkToValue;
	knora-base:subjectClassConstraint language:HumanNaturalLanguageExpression;
	knora-base:objectClassConstraint knora-base:LinkValue.

language:translatedIn
	a owl:ObjectProperty;
	rdfs:label "is translated in"@en, "ist übersetzt in"@de;
	rdfs:comment """Relating a human natural language expression to another one in another natural language it is translated in."""@en;
	rdfs:domain language:HumanNaturalLanguageExpression;
	rdfs:range language:HumanNaturalLanguageExpression;
	rdfs:subPropertyOf knora-base:hasLinkTo;
	knora-base:subjectClassConstraint language:HumanNaturalLanguageExpression;
	knora-base:objectClassConstraint language:Translation.

language:translatedInValue
	a owl:ObjectProperty;
	rdfs:label "is translated in - statement"@en, "ist übersetzt in - Festlegung"@de;
	rdfs:comment """Relating a human natural language expression to a reification statement of the relation between the expression and another one in another natural language it is translated in."""@en;
	rdfs:subPropertyOf knora-base:hasLinkToValue;
	knora-base:subjectClassConstraint language:HumanNaturalLanguageExpression;
	knora-base:objectClassConstraint knora-base:LinkValue.

language:hasTranslator #*
	a owl:ObjectProperty;
	rdfs:label "has translator"@en, "hat Übersetzer"@de;
	rdfs:comment """Relating a natural language expression to an agent that translated it."""@en;
	rdfs:subPropertyOf knora-base:hasLinkTo;
	rdfs:domain language:HumanNaturalLanguageExpression;
	rdfs:range agent:Agent; # [rdfs:subClassOf human:Person, [a owl:Restriction; owl:onProperty agent:hasRole; owl:someValuesFrom language:Translator]];
	knora-base:subjectClassConstraint language:HumanNaturalLanguageExpression;
	knora-base:objectClassConstraint agent:Agent.

language:hasTranslatorValue
	a owl:ObjectProperty;
	rdfs:label "has translator - statement"@en, "hat Übersetzer - Festlegung"@de;
	rdfs:comment """Relating a natural language expression to a reification statement of the relation between the expression and an agent that translated it."""@en;
	rdfs:subPropertyOf knora-base:hasLinkToValue;
	knora-base:subjectClassConstraint language:HumanNaturalLanguageExpression;
	knora-base:objectClassConstraint knora-base:LinkValue.

language:hasPersonTranslator
	a owl:ObjectProperty;
	rdfs:label "has person-translator"@en, "hat Person-Übersetzer"@de;
	rdfs:comment """Relating a natural language expression to a person who translated it."""@en;
	rdfs:domain language:HumanNaturalLanguageExpression;
	rdfs:range human:Person; # [rdfs:subClassOf human:Person, [a owl:Restriction; owl:onProperty human:hasRole; owl:someValuesFrom language:PersonTranslator]];
	rdfs:subPropertyOf language:hasTranslator;
	knora-base:subjectClassConstraint language:HumanNaturalLanguageExpression;
	knora-base:objectClassConstraint human:Person.

language:hasPersonTranslatorValue
	a owl:ObjectProperty;
	rdfs:label "has person-translator - statement"@en, "hat Person-Übersetzer - Festlegung"@de;
	rdfs:comment """Relating a natural language expression to a reification statement of the relation between the expression and a person who translated it."""@en;
	rdfs:subPropertyOf language:hasTranslatorValue;
	knora-base:subjectClassConstraint language:HumanNaturalLanguageExpression;
	knora-base:objectClassConstraint knora-base:LinkValue.

language:hasMachineTranslator
	a owl:ObjectProperty;
	rdfs:label "has machine-translator"@en, "hat Maschine-Übersetzer"@de;
	rdfs:comment """Relating a natural language expression to a machine that translated it."""@en;
	rdfs:domain language:HumanNaturalLanguageExpression;
	rdfs:range device:DigitalElectronicComputer; # [rdfs:subClassOf device:DigitalElectronicComputer, [a owl:Restriction; owl:onProperty human:hasRole; owl:someValuesFrom language:Translator]];
	rdfs:subPropertyOf language:hasTranslator;
	knora-base:subjectClassConstraint language:HumanNaturalLanguageExpression;
	knora-base:objectClassConstraint device:DigitalElectronicComputer.

language:hasMachineTranslatorValue
	a owl:ObjectProperty;
	rdfs:label "has machine-translator - statement"@en, "hat Maschine-Übersetzer - Festlegung"@de;
	rdfs:comment """Relating a natural language expression to a reification statement of the relation between the expression and a machine that translated it."""@en;
	rdfs:subPropertyOf language:hasTranslatorValue;
	knora-base:subjectClassConstraint language:HumanNaturalLanguageExpression;
	knora-base:objectClassConstraint knora-base:LinkValue.

language:translatedInNaturalLanguage
	a owl:ObjectProperty;
	rdfs:label "translated in natural language"@en, "übersetzt in naturlichen Sprache"@de;
	rdfs:comment """Relating a human expression to a natural language wherein it is translated."""@en;
	rdfs:subPropertyOf language:expressedInNaturalLanguage;
	rdfs:domain language:HumanNaturalLanguageExpression;
	rdfs:range language:HumanNaturalLanguage;
	knora-base:subjectClassConstraint language:HumanNaturalLanguageExpression;
	knora-base:objectClassConstraint language:HumanNaturalLanguage.

language:translatedInNaturalLanguageValue
	a owl:ObjectProperty;
	rdfs:label "translated in natural language - statement"@en, "übersetzt in naturlichen Sprache - Festlegung"@de;
	rdfs:comment """Relating a human expression to a reification statement of the relation between the expression and a natural language wherein it is translated."""@en;
	rdfs:subPropertyOf language:expressedInNaturalLanguageValue;
	knora-base:subjectClassConstraint language:HumanNaturalLanguageExpression;
	knora-base:objectClassConstraint knora-base:LinkValue.

language:hasLinguisticComment
	a owl:ObjectProperty;
	rdfs:label "has linguistic comment"@en, "hat linguistischer Kommentar"@de;
	rdfs:comment """Relating a human natural language expression to a linguistic comment (as object) as a textual statement about the resource."""@en;
	rdfs:subPropertyOf text:hasComment;
	knora-base:subjectClassConstraint language:HumanNaturalLanguageExpression;
	knora-base:objectClassConstraint knora-base:TextValue;
	salsah-gui:guiElement salsah-gui:Richtext.