@prefix rdfs: <http://www.w3.org/2000/01/rdf-schema#>.
@prefix owl: <http://www.w3.org/2002/07/owl#>.
@prefix xsd: <http://www.w3.org/2001/XMLSchema#>.
@prefix skos: <http://www.w3.org/2004/02/skos/core#>.
@prefix dct: <http://purl.org/dc/terms/>.
@prefix cidoc: <http://www.cidoc-crm.org/cidoc-crm/>.
@prefix human: <http://www.knora.org/ontology/0048/human#>.
@prefix concept: <http://www.knora.org/ontology/0044/concept#>.
@prefix text: <http://www.knora.org/ontology/0059/text#>.
@prefix knora-base: <http://www.knora.org/ontology/knora-base#>.

@base <http://www.knora.org/ontology/0057/scholasticism>.
@prefix schola: <http://www.knora.org/ontology/0057/scholasticism#>.

<http://www.knora.org/ontology/0057/scholasticism>
	a owl:Ontology;
	dct:title "An ontology about Scholasticism"@en;
	dct:description """Formal description of elements in Scholasticism."""@en;
	dct:creator "Hans Cools, MD, knowledge engineer, ontologist, software developer, NIE, University of Basel, Switzerland"@en;
	dct:contributor "Prof. Dr. Ueli Zahnd, Faculty of Theology, University of Basel, Switzerland"@en, "Gabriel Müller, Faculty of Theology, University of Basel, Switzerland"@en;
	dct:publisher "Basel University, Switzerland"@en;

	knora-base:attachedToProject <http://rdfh.ch/projects/0057>.

#
# CLASSES
#

schola:Scholasticism
	a owl:Class;
	rdfs:label "scholasticism"@en, "Scholastik"@de;
	rdfs:comment """Method of critical thought dominating theological and philosophical study in Western Christianity and teaching by academics or scholastics (schoolmen) of universities in Europe from about 1100 to 1700."""@en;
	rdfs:subClassOf concept:ThoughtMethod. #*

schola:Scholastic
	a owl:Class;
	rdfs:label "scholastic"@en, "ScholastikerIn"@de;
	rdfs:comment """An adherent of Scholasticism."""@en;
	skos:note """There are no female scholastics because women were not allowed to universities."""@en; # Can this be stated that absolute?
	rdfs:subClassOf human:Person, [
#		a owl:Restriction; owl:onProperty schola:hasRole; owl:someValuesFrom schola:Role], [
		a owl:Restriction; owl:onProperty schola:hasRole; owl:minCardinality "0"^^xsd:nonNegativeInteger], [
		a owl:Restriction; owl:onProperty schola:hasRoleValue; owl:minCardinality "0"^^xsd:nonNegativeInteger] #, [
#		a owl:Restriction; owl:onProperty schola:hasReportatorRole; owl:minCardinality "0"^^xsd:nonNegativeInteger], [
#		a owl:Restriction; owl:onProperty schola:hasReportatorRoleValue; owl:minCardinality "0"^^xsd:nonNegativeInteger]
		.

#* schola:Lecture

schola:Role
	a owl:Class;
	rdfs:label "scholastic role"@en;
	rdfs:comment """Role a scholastic has."""@en;
	rdfs:subClassOf human:Role.

schola:Reportator
	a owl:Class;
	rdfs:label "reportator"@la, "reportator"@en, "Reportator"@de;
	rdfs:comment """Role of a scholastic student registering the content of a lesson."""@en; #* also secretary of lecturer, RP
	rdfs:subClassOf schola:Role.

schola:Commentary
	a owl:Class;
	rdfs:label "commentarius scholasticus"@la, "scholastic commentary"@en, "scholastischer Kommentar"@de;
	rdfs:comment """Commentary made by a person with a scholastic role."""@en;
	rdfs:subClassOf text:Commentary, [
		a owl:Restriction; owl:onProperty schola:hasCommentaryMethod; owl:minCardinality "0"^^xsd:nonNegativeInteger], [
		a owl:Restriction; owl:onProperty schola:hasCommentaryMethodValue; owl:minCardinality "0"^^xsd:nonNegativeInteger], [
		a owl:Restriction; owl:onProperty schola:hasCommentaryForm; owl:minCardinality "0"^^xsd:nonNegativeInteger], [
		a owl:Restriction; owl:onProperty schola:hasCommentaryFormValue; owl:minCardinality "0"^^xsd:nonNegativeInteger]. #, [
#		a owl:Restriction; owl:onProperty schola:hasReportator; owl:minCardinality "0"^^xsd:nonNegativeInteger], [
#		a owl:Restriction; owl:onProperty schola:hasReportatorValue; owl:minCardinality "0"^^xsd:nonNegativeInteger] #, [
#		a owl:Restriction; owl:onProperty text:hasTitle; owl:minCardinality "0"^^xsd:nonNegativeInteger], [				#* + rest
#		a owl:Restriction; owl:onProperty text:hasAlias; owl:minCardinality "0"^^xsd:nonNegativeInteger], [
#		a owl:Restriction; owl:onProperty text:hasDescription; owl:minCardinality "0"^^xsd:nonNegativeInteger], [
#		a owl:Restriction; owl:onProperty text:hasIncipit; owl:minCardinality "0"^^xsd:nonNegativeInteger], [
#		a owl:Restriction; owl:onProperty text:hasExplicit; owl:minCardinality "0"^^xsd:nonNegativeInteger], [
#		a owl:Restriction; owl:onProperty text:hasAuthor; owl:minCardinality "0"^^xsd:nonNegativeInteger], [
#		a owl:Restriction; owl:onProperty text:hasAuthorValue; owl:minCardinality "0"^^xsd:nonNegativeInteger], [
#		a owl:Restriction; owl:onProperty text:hasRevisor; owl:minCardinality "0"^^xsd:nonNegativeInteger], [
#		a owl:Restriction; owl:onProperty text:hasRevisorValue; owl:minCardinality "0"^^xsd:nonNegativeInteger], [
#		a owl:Restriction; owl:onProperty textedit:hasEditor; owl:minCardinality "0"^^xsd:nonNegativeInteger], [
#		a owl:Restriction; owl:onProperty textedit:hasEditorValue; owl:minCardinality "0"^^xsd:nonNegativeInteger], [
#		a owl:Restriction; owl:onProperty textedit:hasAbbreviator; owl:minCardinality "0"^^xsd:nonNegativeInteger], [
#		a owl:Restriction; owl:onProperty textedit:hasAbbreviatorValue; owl:minCardinality "0"^^xsd:nonNegativeInteger], [
#		a owl:Restriction; owl:onProperty textedit:hasGlossator; owl:minCardinality "0"^^xsd:nonNegativeInteger], [
#		a owl:Restriction; owl:onProperty textedit:hasGlossatorValue; owl:minCardinality "0"^^xsd:nonNegativeInteger], [
#		a owl:Restriction; owl:onProperty textedit:hasRedactor; owl:minCardinality "0"^^xsd:nonNegativeInteger], [
#		a owl:Restriction; owl:onProperty textedit:hasRedactorValue; owl:minCardinality "0"^^xsd:nonNegativeInteger]
#		a owl:Restriction; owl:onProperty human:hasCreating; owl:minCardinality "0"^^xsd:nonNegativeInteger], [
#		a owl:Restriction; owl:onProperty human:hasCreatingValue; owl:minCardinality "0"^^xsd:nonNegativeInteger], [
#		a owl:Restriction; owl:onProperty human:hasCreationDate; owl:minCardinality "0"^^xsd:nonNegativeInteger], [
#		.

schola:CommentaryMethod #* stage?, RP
	a owl:Class;
	rdfs:label "scholastic commentary method"@en, "scholastische Kommentarmethode"@de;
	rdfs:comment """Scholastic method to comment."""@en;
	rdfs:subClassOf concept:Procedure.

schola:Lectura
	a owl:Class;
	rdfs:label "lectura"@la;
	rdfs:comment """Scholastic commentary on a text as presented by its author in a lecture."""@en;
	rdfs:subClassOf schola:CommentaryMethod.

schola:LecturaRevisa #* = Ordinatio ?, RP
	a owl:Class;
	rdfs:label "lectura revisa"@la;
	rdfs:comment """Scholastic commentary on a text as revised by its author after its presentation in a lecture."""@en;
	rdfs:subClassOf schola:CommentaryMethod.

schola:Reportatio
	a owl:Class;
	rdfs:label "reportatio"@la;
	rdfs:comment """Scholastic commentary on a text as recorded by a student."""@en; #* "listener", "auditor" instead of "student"?
	rdfs:subClassOf schola:CommentaryMethod.

schola:ReportatioApprobata
	a owl:Class;
	rdfs:label "reportatio approbata"@la;
	rdfs:comment """Scholastic commentary on a text as student recordings approved by the master."""@en;
	rdfs:subClassOf schola:CommentaryMethod.

schola:Ordinatio
	a owl:Class;
	rdfs:label "ordinatio"@la;
	rdfs:comment """Scholastic commentary on a text as composed for publication."""@en;
	rdfs:subClassOf schola:CommentaryMethod.

schola:CommentaryForm
	a owl:Class;
	rdfs:label "scholastic commentary form"@en, "scholastische Kommentarform"@de;
	rdfs:comment """Form to represent a scholastic commentary."""@en;
	rdfs:subClassOf concept:Information.

schola:CommentaryGlosses # note structure
	a owl:Class;
	rdfs:label "glosses"@en, "Glossen"@de;
	rdfs:comment """Scholastic commentary on a text in the form of an added text or gloss."""@en;
	rdfs:subClassOf schola:CommentaryForm.

schola:CommentaryLiteralExposition # ?
	a owl:Class;
	rdfs:label "literal exposition"@en, "wörtliche Auslegung"@de;
	rdfs:comment """Scholastic commentary on a text in the form of a literal exposition."""@en;
	rdfs:subClassOf schola:CommentaryForm.

schola:CommentaryQuestions # speech act
	a owl:Class;
	rdfs:label "questions"@en, "Fragen"@de;
	rdfs:comment """Scholastic commentary on a text in the form of questions."""@en;	# not linked to content ?
	rdfs:subClassOf schola:CommentaryForm.

schola:CommentaryAbbreviation # edition
	a owl:Class;
	rdfs:label "abbreviation"@en, "Kurzfassung"@de;
	rdfs:comment """Scholastic commentary on a text in the form of a shortened version."""@en;
	rdfs:subClassOf schola:CommentaryForm.

schola:CommentaryParaphrase # edition
	a owl:Class;
	rdfs:label "paraphrase"@en, "Paraphrase"@de;
	rdfs:comment """Scholastic commentary on a text in the form of a restatement of a text to clarify meaning."""@en;
	rdfs:subClassOf schola:CommentaryForm.

schola:CommentaryTable # structure
	a owl:Class;
	rdfs:label "table"@en, "Tabelle"@de;
	rdfs:comment """Scholastic commentary on a text in the form of condensed information in a table."""@en;
	rdfs:subClassOf schola:CommentaryForm.

schola:CommentaryVerse # structure
	a owl:Class;
	rdfs:label "metric"@en, "Versform"@de; #*
	rdfs:comment """Scholastic commentary on a text in the form of condensing information in verse form."""@en;
	rdfs:subClassOf schola:CommentaryForm.

schola:CommentarySyllogisms
	a owl:Class;
	rdfs:label "syllogisms"@en, "Syllogismen"@de;
	rdfs:comment """Scholastic commentary on a text in the form of syllogisms."""@en;
	rdfs:subClassOf schola:CommentaryForm.

schola:CommentaryConclusion
	a owl:Class;
	rdfs:label "conclusions"@en, "Schlussfolgerungen"@de;
	rdfs:comment """Scholastic commentary on a text in the form of conclusions."""@en;
	rdfs:subClassOf schola:CommentaryForm.

#
# PROPERTIES
#

schola:hasRole
	a owl:ObjectProperty;
	rdfs:label "has role"@en, "hat Rolle"@de;
	rdfs:comment """Relating a scholastic to a role he has."""@en;
	rdfs:domain schola:Scholastic;
	rdfs:range schola:Role;
	rdfs:subPropertyOf human:hasRole;
	knora-base:subjectClassConstraint schola:Scholastic;
	knora-base:objectClassConstraint schola:Role.

schola:hasRoleValue
	a owl:ObjectProperty;
	rdfs:label "has role - statement"@en, "hat Rolle - Festlegung"@de;
	rdfs:comment """Relating a scholastic to a statement as reification of the relation between the scholastic and a role he has."""@en;
	rdfs:subPropertyOf human:hasRoleValue;
	knora-base:subjectClassConstraint schola:Scholastic;
	knora-base:objectClassConstraint knora-base:LinkValue.

# schola:hasReportatorRole
#	a owl:ObjectProperty;
#	rdfs:label "has reportator role"@en, "hat Reportator Rolle"@de;
#	rdfs:comment """Relating a scholastic to a reportator role he has."""@en;
#	rdfs:domain schola:Scholastic;
#	rdfs:range schola:Reportator;  
#	rdfs:subPropertyOf schola:hasRole;
#	knora-base:subjectClassConstraint schola:Scholastic;
#	knora-base:objectClassConstraint schola:Reportator.

# schola:hasReportatorRoleValue
#	a owl:ObjectProperty;
#	rdfs:label "has reportator role - statement"@en, "hat Reportator Rolle - Festlegung"@de;
#	rdfs:comment """Relating a scholastic to a statement as reification of the relation between the scholastic and a reportator role he has."""@en;
#	rdfs:subPropertyOf schola:hasRoleValue;
#	knora-base:subjectClassConstraint schola:Scholastic;
#	knora-base:objectClassConstraint knora-base:LinkValue.

#schola:hasReportator
#	a owl:ObjectProperty;
#	rdfs:label "has reportator"@en, "hat Reportator"@de;
#	rdfs:comment """Relating a scholastic lecture to a scholastic who reported it."""@en;
#	rdfs:domain schola:Lecture;
#	rdfs:range schola:Scholastic;  
#	rdfs:subPropertyOf knora-base:hasLinkTo;
#	knora-base:subjectClassConstraint schola:Lecture;
#	knora-base:objectClassConstraint schola:Scholastic.

#schola:hasReportatorValue
#	a owl:ObjectProperty;
#	rdfs:label "has reportator - statement"@en, "hat Reportator - Festlegung"@de;
#	rdfs:comment """Relating a scholastic lecture to a statement as reification of the relation between the lecture and a scholastic who reported it."""@en;
#	rdfs:subPropertyOf knora-base:hasLinkToValue;
#	knora-base:subjectClassConstraint schola:Lecture;
#	knora-base:objectClassConstraint knora-base:LinkValue.

schola:hasCommentaryMethod
	a owl:ObjectProperty;
	rdfs:label "has commentary method"@en, "hat Kommentarmethode"@de;
	rdfs:comment """Relating a scholastic commentary to a method it adheres to."""@en;
	rdfs:subPropertyOf knora-base:hasLinkTo;
	knora-base:subjectClassConstraint schola:Commentary;
	knora-base:objectClassConstraint schola:CommentaryMethod.

schola:hasCommentaryMethodValue
	a owl:ObjectProperty;
	rdfs:label "has commentary method - statement"@en, "hat Kommentarmethode - Festlegung"@de;
	rdfs:comment """Relating a scholastic commentary to a statement as reification of the relation between the scholastic commentary and a method it adheres to."""@en;
	rdfs:subPropertyOf knora-base:hasLinkToValue;
	knora-base:subjectClassConstraint schola:Commentary;
	knora-base:objectClassConstraint knora-base:LinkValue.

schola:hasCommentaryForm
	a owl:ObjectProperty;
	rdfs:label "has commentary form"@en, "hat Kommentarform"@de;
	rdfs:comment """Relating a scholastic commentary to a form it is represented in."""@en;
	rdfs:subPropertyOf knora-base:hasLinkTo;
	knora-base:subjectClassConstraint schola:Commentary;
	knora-base:objectClassConstraint schola:CommentaryForm.

schola:hasCommentaryFormValue
	a owl:ObjectProperty;
	rdfs:label "has commentary form - statement"@en, "hat Kommentarform - Festlegung"@de;
	rdfs:comment """Relating a scholastic commentary to a statement as reification of the relation between the scholastic commentary and a form it is represented in."""@en;
	rdfs:subPropertyOf knora-base:hasLinkToValue;
	knora-base:subjectClassConstraint schola:Commentary;
	knora-base:objectClassConstraint knora-base:LinkValue.

# schola:commentaryHasTable etc.