@prefix rdfs: <http://www.w3.org/2000/01/rdf-schema#>.
@prefix owl: <http://www.w3.org/2002/07/owl#>.
@prefix xsd: <http://www.w3.org/2001/XMLSchema#>.
@prefix skos: <http://www.w3.org/2004/02/skos/core#>.
@prefix dct: <http://purl.org/dc/terms/>.
@prefix foaf: <http://xmlns.com/foaf/0.1/>.
@prefix cidoc: <http://www.cidoc-crm.org/cidoc-crm/>.
@prefix frbroo: <http://iflastandards.info/ns/fr/frbr/frbroo/>.
@prefix event: <http://www.knora.org/ontology/0047/event#>.
@prefix human: <http://www.knora.org/ontology/0048/human#>.
@prefix language: <http://www.knora.org/ontology/004F/language#>.
@prefix concept: <http://www.knora.org/ontology/0044/concept#>.
@prefix text: <http://www.knora.org/ontology/0059/text#>.
@prefix text-structure: <http://www.knora.org/ontology/005B/text-structure#>.
@prefix infocar: <http://www.knora.org/ontology/004C/information-carrier#>.
@prefix publish: <http://www.knora.org/ontology/0056/publishing#>.
@prefix litera: <http://www.knora.org/ontology/0050/literature#>.
@prefix knora-base: <http://www.knora.org/ontology/knora-base#>.
@prefix salsah-gui: <http://www.knora.org/ontology/salsah-gui#>.

@base <http://www.knora.org/ontology/005A/text-editing>.
@prefix textedit: <http://www.knora.org/ontology/005A/text-editing#>.

<http://www.knora.org/ontology/005A/text-editing>
	a owl:Ontology;
	dct:title "An ontology about text editing"@en;
	dct:description """Formal description of text editing, general subclasses, related classes, and properties."""@en;
	dct:creator "Hans Cools, MD, knowledge engineer, ontologist, software developer, NIE-INE, Basel University, Switzerland"@en;
	dct:contributor "Roberta Padlina, tool coordinator, NIE-INE, Basel University, Switzerland"@en;
	dct:publisher "Basel University, Switzerland"@en;
#	rdfs:seeAlso <https://digitallatin.github.io/guidelines/LDLT-Guidelines.html>;

	knora-base:attachedToProject <http://rdfh.ch/projects/005A>.

textedit:Derivative #*
	a owl:Class;
	rdfs:label "text derivative"@en, "abgeleitete Text"@de;
	rdfs:comment """Text expression derived from another text expression."""@en;
	rdfs:subClassOf text:Expression, human:CreationDerivative, [
		a owl:Restriction; owl:onProperty textedit:hasDiacriticalSign; owl:minCardinality "0"^^xsd:nonNegativeInteger], [
		a owl:Restriction; owl:onProperty textedit:hasPageIndicator; owl:minCardinality "0"^^xsd:nonNegativeInteger], [
		a owl:Restriction; owl:onProperty textedit:hasPageNumberIndicator; owl:minCardinality "0"^^xsd:nonNegativeInteger], [
		a owl:Restriction; owl:onProperty textedit:hasColumnIndicator; owl:minCardinality "0"^^xsd:nonNegativeInteger].

textedit:Edition # can be on >= 1 carrier
	a owl:Class;
	rdfs:label "text edition"@en, "Text-Edition"@de; # Lesetext subClassOf
	rdfs:comment """Changed form of a text expression as a result of editing."""@en; #* drop expression?
	rdfs:subClassOf textedit:Derivative.

textedit:Editor
	a owl:Class;
	rdfs:label "text editor"@en, "Text-Redakteur"@de;
	rdfs:comment """Role of a person changing a text."""@en;
	rdfs:subClassOf human:Creator.

textedit:Redactor #* -> scholastic?
	a owl:Class;
	rdfs:label "redactor"@la, "redactor"@en, "Redactor"@de;
	rdfs:comment """Editor assembling parts of texts to a new coherent text."""@en;
	rdfs:subClassOf textedit:Editor.

textedit:Glossator #* -> scholastic?
	a owl:Class;
	rdfs:label "glossator"@la, "glossator"@en, "Glossator"@de;
	rdfs:comment """Editor adding glosses to a text."""@en;
	rdfs:subClassOf textedit:Editor.

textedit:Abbreviator #* -> scholastic?
	a owl:Class;
	rdfs:label "abbreviator"@la, "abbreviator"@en, "Abkürzer"@de;
	rdfs:comment """Editor shortening a text."""@en;
	rdfs:subClassOf textedit:Editor.

# genetic edition: description of edition of another

textedit:DiplomaticTranscription
	a owl:Class;
	rdfs:label "diplomatic transcription"@en, "diplomatische Umschrift"@de;
	rdfs:comment """Transcription of a text with diacritical signs indicating visual textual properties to describe the textual state."""@en;
#	skos:note """only autographs or jurudical; without interpretation""";
	rdfs:subClassOf textedit:Derivative, [
		a owl:Restriction; owl:onProperty textedit:isDiplomaticTranscriptionOfTextOnPage; owl:minCardinality "0"^^xsd:nonNegativeInteger], [
		a owl:Restriction; owl:onProperty textedit:isDiplomaticTranscriptionOfTextOnPageValue; owl:minCardinality "0"^^xsd:nonNegativeInteger]#, [
#		a owl:Restriction; owl:onProperty infocar:isOnCarrier; owl:cardinality "1"^^xsd:nonNegativeInteger], [
#		a owl:Restriction; owl:onProperty infocar:isOnCarrierValue; owl:cardinality "1"^^xsd:nonNegativeInteger]
		.

textedit:CriticalEdition
	a owl:Class;
	rdfs:label "critical text edition"@en, "kritische Textedition"@de; #* kanonische Textfassung
	rdfs:comment """Edition to which an editor added evidence and interpretation of a text creation and historical transmission, allowing readers to assess the editor's choice."""@en; #*
	rdfs:subClassOf textedit:Edition, [ #* + argumentation and discussing other edition
#		a owl:Restriction; owl:onProperty textedit:hasApparatus; owl:someValuesFrom textedit:CriticalApparatus], [
		a owl:Restriction; owl:onProperty textedit:hasApparatus; owl:minCardinality "1"^^xsd:nonNegativeInteger], [
		a owl:Restriction; owl:onProperty textedit:hasApparatusValue; owl:minCardinality "1"^^xsd:nonNegativeInteger].

textedit:GeneticEdition
	a owl:Class;
	rdfs:label "genetic edition"@en, "genetische Edition"@de, "édition génétique"@fr, "edizione genetica"@it;
	rdfs:comment """Critical edition accounting for the modifications by the author."""@en;
	rdfs:subClassOf textedit:CriticalEdition.

textedit:CriticalApparatus
	a owl:Class;
	rdfs:label "critical apparatus"@en, "textkritischer Apparat"@de, "apparatus criticus"@la;
	rdfs:comment """Note to a critical text edition providing information of a textual version."""@en; #* more than note
	rdfs:subClassOf text:Expression #, [
#		a owl:Restriction; owl:onProperty textedit:isApparatusOf; owl:minCardinality "0"^^xsd:nonNegativeInteger], [
#		a owl:Restriction; owl:onProperty textedit:isApparatusOfValue; owl:minCardinality "0"^^xsd:nonNegativeInteger]#, [
#		a owl:Restriction; owl:onProperty text-structure:hasStructure; owl:allValuesFrom text-structure:NoteStructure], [
#		a owl:Restriction; owl:onProperty text-structure:hasStructure; owl:minCardinality "0"^^xsd:nonNegativeInteger], [
#		a owl:Restriction; owl:onProperty text-structure:hasStructureValue; owl:minCardinality "0"^^xsd:nonNegativeInteger]
		.

# apparatus has format:
# eg.
# location of version in text
# lemma: part of text in CA
# symbol
# source
# list of variants + source: if frequently cited: abbreviated with a siglum

textedit:ApparatusFontium
	a owl:Class;
	rdfs:label "apparatus fontium"@en, "apparatus fontium"@de, "apparatus fontium"@la;
	rdfs:comment """Critical apparatus containing references to texts quoted or cited [?dif] by the author [of the original?] in the text of the cr. edition."""@en;
	rdfs:subClassOf textedit:CriticalApparatus.

textedit:Reading #* bound to certain period?
	a owl:Class;
	rdfs:label "reading"@en, "Textinterpretation"@de, "lezione"@it, "lectio"@la; #*
	rdfs:comment """Reading of the text in one given witness."""@en; #* text? # spezifische Interpretation eines Textes
	rdfs:subClassOf text:Expression. #*

textedit:Lemma #* structure, but specific for editing?
	a owl:Class;
	rdfs:label "lemma"@en, "Lemma"@de, "lemma"@it;
	rdfs:comment """A word or phrase *or the absence thereof* judged by an editor to be authentic, accurate, and/or authoritative; making up the edited text of a critical edition."""@en; #* dif word - phrase
	rdfs:subClassOf textedit:Reading. #* -> part of OR unit of CA

#* (oder Stichwort) ist in der Editionswissenschaft das Wort im Haupttext, auf welches sich die Anmerkung oder der textkritische Apparat eines Kommentars bezieht

#* linguistics: morphology and lexicography, a lemma (plural lemmas or lemmata) is the canonical form
#* morphology: study of words, how they are formed, and their relationship to other words in the same language
#* lexikographisch: grundform eines Wortes

textedit:Variant
	a owl:Class;
	rdfs:label "variant"@en, "Variant"@de, "variante"@it;
	rdfs:comment """A word or phrase *or the absence thereof* judged by an editor to be unsatisfactory for linguistic and/or stylistic reasons, but of interest for establishing the text; varying from what the editor has judged to be the lemma."""@en;
	rdfs:subClassOf textedit:Reading. #* -> part of OR unit of CA
	  
textedit:Emendation
	a owl:Class;
	rdfs:label "emendation"@en, "emendazione"@it;
	rdfs:comment """A reading expressly proposed by some person (possibly the editor) and accepted by the editor into the main text of an edition."""@en;
	rdfs:subClassOf textedit:Reading.
	# OR
	# rdfs:comment """A reading based on a conjecture and that is used to correct the text of an edition."""@en;
	# then: rdfs:subClassOf textedit:Conjecture + restriction: is integrated in the main text of an edition.
	# see:
	# This distinction between "emendation” and "conjecture" supports the goal of these guidelines of drawing attention to editions as arguments. 
	# The terms are used subjectively, with regard to a particular edition. Readers of an edition may agree or disagree about whether a particular reading emends the text, 
	# but the editor's argument is that a reading either emends the text, in which case it is an emendation, or does not in which case it is a conjecture.

textedit:Conjecture #* conjectural emendation
	a owl:Class;
	rdfs:label "conjecture"@en, "Konjektur"@de, "?"@it;
	rdfs:comment """A reading expressly proposed  - possibly the editor [?] - *and determined by* an editor to be of interest in establishing the text, but not to be printed in the main text of the edition."""@en;
	# rdfs:comment """A reading choosed by an editor after some reasoning or deduction, but which isn't attested in any of the manuscripts."""@en;
	rdfs:subClassOf textedit:Reading.

# OD: suggestion of a reading of a text not present in the original source

#
# PROPERTIES
#

textedit:hasEditor
	a owl:ObjectProperty;
	rdfs:label "has editor"@en, "hat Text-Redakteur"@de;
	rdfs:comment """Relating a text expression to a person who edited it."""@en;
	rdfs:domain text:Expression;
#	rdfs:range [rdfs:subClassOf human:Person, [a owl:Restriction; owl:onProperty human:hasRole; owl:someValuesFrom textedit:Editor]];
	rdfs:subPropertyOf knora-base:hasLinkTo;
	knora-base:subjectClassConstraint text:Expression;
	knora-base:objectClassConstraint human:Person.

textedit:hasEditorValue
	a owl:ObjectProperty;
	rdfs:label "has editor - statement"@en, "hat Text-Redakteur - Festlegung"@de;
	rdfs:comment """Relating a text expression to a reification statement of the relation between the text and a person who edited it."""@en;
	rdfs:subPropertyOf knora-base:hasLinkToValue;
	knora-base:subjectClassConstraint text:Expression;
	knora-base:objectClassConstraint knora-base:LinkValue.

textedit:hasRedactor
	a owl:ObjectProperty;
	rdfs:label "has redactor"@en, "hat Redaktor"@de;
	rdfs:comment """Relating a text expression to a person who redacted it."""@en;
	rdfs:domain text:Expression;
#	rdfs:range [rdfs:subClassOf human:Person, [a owl:Restriction; owl:onProperty human:hasRole; owl:someValuesFrom textedit:Redactor]];
	rdfs:subPropertyOf knora-base:hasLinkTo;
	knora-base:subjectClassConstraint text:Expression;
	knora-base:objectClassConstraint human:Person.

textedit:hasRedactorValue
	a owl:ObjectProperty;
	rdfs:label "has redactor - statement"@en, "hat Redaktor - Festlegung"@de;
	rdfs:comment """Relating a text expression to a reification statement of the relation between the text and a person who redacted it."""@en;
	rdfs:subPropertyOf knora-base:hasLinkToValue;
	knora-base:subjectClassConstraint text:Expression;
	knora-base:objectClassConstraint knora-base:LinkValue.

textedit:hasGlossator
	a owl:ObjectProperty;
	rdfs:label "has glossator"@en, "hat Glossator"@de;
	rdfs:comment """Relating a text expression to a person who glossed it."""@en;
	rdfs:domain text:Expression;
#	rdfs:range [rdfs:subClassOf human:Person, [a owl:Restriction; owl:onProperty human:hasRole; owl:someValuesFrom text:Glossator]];
	rdfs:subPropertyOf knora-base:hasLinkTo;
	knora-base:subjectClassConstraint text:Expression;
	knora-base:objectClassConstraint human:Person.

textedit:hasGlossatorValue
	a owl:ObjectProperty;
	rdfs:label "has glossator - statement"@en, "hat Glossator - Festlegung"@de;
	rdfs:comment """Relating a text expression to a reification statement of the relation between the text and a person who glossed it."""@en;
	rdfs:subPropertyOf knora-base:hasLinkToValue;
	knora-base:subjectClassConstraint text:Expression;
	knora-base:objectClassConstraint knora-base:LinkValue.

textedit:hasAbbreviator
	a owl:ObjectProperty;
	rdfs:label "has abbreviator"@en, "hat Abkurzer"@de;
	rdfs:comment """Relating a text expression to a person who abbreviated it."""@en;
	rdfs:domain text:Expression;
#	rdfs:range [rdfs:subClassOf human:Person, [a owl:Restriction; owl:onProperty human:hasRole; owl:someValuesFrom text:Abbreviator]];
	rdfs:subPropertyOf knora-base:hasLinkTo;
	knora-base:subjectClassConstraint text:Expression;
	knora-base:objectClassConstraint human:Person.

textedit:hasAbbreviatorValue
	a owl:ObjectProperty;
	rdfs:label "has abbreviator - statement"@en, "hat Abkurzer - Festlegung"@de;
	rdfs:comment """Relating a text to expression a reification statement of the relation between the text and a person who abbreviated it."""@en;
	rdfs:subPropertyOf knora-base:hasLinkToValue;
	knora-base:subjectClassConstraint text:Expression;
	knora-base:objectClassConstraint knora-base:LinkValue.

textedit:hasEdition
	a owl:ObjectProperty;
	rdfs:label "has edition"@en, "hat Edition"@de;
	rdfs:comment "Relating a text to an edition thereof."@en;
	rdfs:domain text:Expression;
	rdfs:range textedit:Edition;
	rdfs:subPropertyOf knora-base:hasLinkTo;
	knora-base:subjectClassConstraint text:Expression;
	knora-base:objectClassConstraint textedit:Edition.

textedit:hasEditionValue
	a owl:ObjectProperty;
	rdfs:label "has edition - statement"@en, "hat Edition - Festlegung"@de;
	rdfs:comment "Relating a text to a reification statement of the relation between the text and an edition thereof."@en;
	rdfs:subPropertyOf knora-base:hasLinkToValue;
	knora-base:subjectClassConstraint text:Expression;
	knora-base:objectClassConstraint knora-base:LinkValue.

#:hasEditedContent
#	a owl:ObjectProperty;
#	rdfs:label "has edited content"@en;
#	rdfs:comment """Relating an edition to its content (as object)."""@en;
#	rdfs:subPropertyOf language:hasContent;
#	knora-base:subjectClassConstraint textedit:Edition;
#	knora-base:objectClassConstraint knora-base:TextValue;
#	salsah-gui:guiElement salsah-gui:Richtext.

textedit:hasSameEditionAs # different from https://www.w3.org/TR/owl-ref/#sameAs-def
	a owl:ObjectProperty;
	rdfs:label "has same edition as"@en, "hat gleiche Edition als"@de;
	rdfs:comment """Relating two texts with a same edition."""@en;
	rdfs:subPropertyOf knora-base:hasLinkTo;
	knora-base:subjectClassConstraint text:Expression;
	knora-base:objectClassConstraint text:Expression.

textedit:hasSameEditionAsValue
	a owl:ObjectProperty;
	rdfs:label "has same edition as - statement"@en, "hat gleiche Edition als - Festlegung"@de;
	rdfs:comment """Relating a text to a reification statement of the relation between the text and another one with a same edition."""@en;
	rdfs:subPropertyOf knora-base:hasLinkToValue;
	knora-base:subjectClassConstraint text:Expression;
	knora-base:objectClassConstraint knora-base:LinkValue.

textedit:hasDiplomaticTranscription
	a owl:ObjectProperty;
	rdfs:label "has diplomatic transcription"@en, "hat diplomatische Umschrift"@de;
	rdfs:comment "Relating a text to a diplomatic transcription thereof."@en;
	rdfs:subPropertyOf knora-base:hasLinkTo;
	knora-base:subjectClassConstraint text:Expression;
	knora-base:objectClassConstraint textedit:DiplomaticTranscription.

textedit:hasDiplomaticTranscriptionValue
	a owl:ObjectProperty;
	rdfs:label "has diplomatic transcription - statement"@en, "hat diplomatische Umschrift - Festlegung"@de;
	rdfs:comment "Relating a text to a reification statement of the relation between the text and a diplomatic transcription thereof."@en;
	rdfs:subPropertyOf knora-base:hasLinkToValue;
	knora-base:subjectClassConstraint text:Expression;
	knora-base:objectClassConstraint knora-base:LinkValue.

textedit:isDiplomaticTranscriptionOfTextOnPage
	a owl:ObjectProperty;
	rdfs:label "is diplomatic transcription of text on page"@en, "ist diplomatische Umschrift des Textes auf Seite"@de;
	rdfs:comment "Relating a diplomatic transcription to a page its source text is on."@en;
	rdfs:domain textedit:DiplomaticTranscription;
	rdfs:range infocar:Page;
	rdfs:subPropertyOf knora-base:hasLinkTo;
	knora-base:subjectClassConstraint textedit:DiplomaticTranscription;
	knora-base:objectClassConstraint infocar:Page.

textedit:isDiplomaticTranscriptionOfTextOnPageValue
	a owl:ObjectProperty;
	rdfs:label "is diplomatic transcription of text on page - statement"@en, "ist diplomatische Umschrift des Textes auf Seite - Festlegung"@de;
	rdfs:comment "Relating a diplomatic transcription to a reification statement of the relation between the diplomatic transcription and a page its source text is on."@en;
	rdfs:subPropertyOf knora-base:hasLinkToValue;
	knora-base:subjectClassConstraint textedit:DiplomaticTranscription;
	knora-base:objectClassConstraint knora-base:LinkValue.

textedit:hasCriticalEdition
	a owl:ObjectProperty;
	rdfs:label "has critical text edition"@en, "hat kritische Textedition"@de;
	rdfs:comment "Relating a text expression to a critical edition thereof."@en;
	rdfs:domain text:Expression;
	rdfs:range textedit:CriticalEdition;
	rdfs:subPropertyOf textedit:hasEdition;
	knora-base:subjectClassConstraint text:Expression;
	knora-base:objectClassConstraint textedit:CriticalEdition.

textedit:hasCriticalEditionValue
	a owl:ObjectProperty;
	rdfs:label "has critical text edition - statement"@en, "hat kritische Textedition - Festlegung"@de;
	rdfs:comment "Relating a text expression to a reification statement of the relation between the text and a critical edition thereof."@en;
	rdfs:subPropertyOf textedit:hasEditionValue;
	knora-base:subjectClassConstraint text:Expression;
	knora-base:objectClassConstraint knora-base:LinkValue.

textedit:hasDiacriticalSign
	a owl:ObjectProperty;
	rdfs:label "has diacritical sign"@en, "hat diakritisches Zeichen"@de;
	rdfs:comment """Relating a derived text expression to a sign (as object) indicating a textual aspect of the original text."""@en;
	rdfs:subPropertyOf language:hasContent;
	knora-base:subjectClassConstraint textedit:Derivative;
	knora-base:objectClassConstraint knora-base:TextValue;
	salsah-gui:guiElement salsah-gui:Richtext.

textedit:hasPageIndicator
	a owl:ObjectProperty;
	rdfs:label "has page indicator"@en, "hat Seite-Indikator"@de;
	rdfs:comment """Relating a derived text expression to a diacritical sign (as object) that indicates where a page starts."""@en;
	rdfs:subPropertyOf textedit:hasDiacriticalSign;
	knora-base:subjectClassConstraint textedit:Derivative;
	knora-base:objectClassConstraint knora-base:TextValue;
	salsah-gui:guiElement salsah-gui:Richtext.

textedit:hasPageNumberIndicator
	a owl:ObjectProperty;
	rdfs:label "has page number indicator"@en, "hat Seitennummer-Indikator"@de;
	rdfs:comment """Relating a derived text expression to a diacritical sign (as object) that indicates the number of a page."""@en;
	rdfs:subPropertyOf textedit:hasDiacriticalSign;
	knora-base:subjectClassConstraint textedit:Derivative;
	knora-base:objectClassConstraint knora-base:TextValue;
	salsah-gui:guiElement salsah-gui:Richtext.

textedit:hasColumnIndicator
	a owl:ObjectProperty;
	rdfs:label "has column indicator"@en, "hat Spalte-Indikator"@de;
	rdfs:comment """Relating a derived text expression to a diacritical sign (as object) that indicates where on a page a column starts."""@en;
	rdfs:subPropertyOf textedit:hasDiacriticalSign;
	knora-base:subjectClassConstraint textedit:Derivative;
	knora-base:objectClassConstraint knora-base:TextValue;
	salsah-gui:guiElement salsah-gui:Richtext.

textedit:hasApparatus
	a owl:ObjectProperty;
	rdfs:label "has apparatus of"@en, "hat Apparat"@de;
	rdfs:comment """Relating a critical edition to its apparatus."""@en;
	rdfs:domain textedit:CriticalEdition;
	rdfs:range textedit:CriticalApparatus;
	rdfs:subPropertyOf knora-base:hasLinkTo;
	knora-base:subjectClassConstraint textedit:CriticalEdition;
	knora-base:objectClassConstraint textedit:CriticalApparatus.

textedit:hasApparatusValue
	a owl:ObjectProperty;
	rdfs:label "has apparatus - statement"@en, "hat Apparat - Festlegung"@de;
	rdfs:comment """Relating a critical edition to a reification statement of the relation between the edition and its apparatus."""@en;
	rdfs:subPropertyOf knora-base:hasLinkToValue;
	knora-base:subjectClassConstraint textedit:CriticalEdition;
	knora-base:objectClassConstraint knora-base:LinkValue.

#textedit:isApparatusOf
#	a owl:ObjectProperty;
#	rdfs:label "is apparatus of"@en, "ist Apparat von"@de;
#	rdfs:comment """Relating a critical apparatus to its critical edition."""@en;
#	rdfs:domain textedit:CriticalApparatus;
#	rdfs:range textedit:CriticalEdition;
#	rdfs:subPropertyOf concept:isPartOf;
#	knora-base:subjectClassConstraint textedit:CriticalApparatus;
#	knora-base:objectClassConstraint textedit:CriticalEdition.

#textedit:isApparatusOfValue
#	a owl:ObjectProperty;
#	rdfs:label "is apparatus of - statement"@en, "ist Apparat von - Festlegung"@de;
#	rdfs:comment """Relating a critical apparatus to a reification statement of the relation between the apparatus and its critical edition."""@en;
#	rdfs:subPropertyOf concept:isPartOfValue;
#	knora-base:subjectClassConstraint textedit:CriticalApparatus;
#	knora-base:objectClassConstraint knora-base:LinkValue.