@prefix rdfs: <http://www.w3.org/2000/01/rdf-schema#>.
@prefix owl: <http://www.w3.org/2002/07/owl#>.
@prefix xsd: <http://www.w3.org/2001/XMLSchema#>.
@prefix skos: <http://www.w3.org/2004/02/skos/core#>.
@prefix dct: <http://purl.org/dc/terms/>.
@prefix foaf: <http://xmlns.com/foaf/0.1/>.
@prefix cidoc: <http://www.cidoc-crm.org/cidoc-crm/>.
@prefix frbroo: <http://iflastandards.info/ns/fr/frbr/frbroo/>.
@prefix event: <http://www.knora.org/ontology/0047/event#>.
@prefix human: <http://www.knora.org/ontology/0048/human#>.
@prefix language: <http://www.knora.org/ontology/004F/language#>.
@prefix concept: <http://www.knora.org/ontology/0044/concept#>.
@prefix text-structure: <http://www.knora.org/ontology/005B/text-structure#>.
@prefix textedit: <http://www.knora.org/ontology/005A/text-editing#>.
@prefix infocar: <http://www.knora.org/ontology/004C/information-carrier#>.
@prefix publish: <http://www.knora.org/ontology/0056/publishing#>.
@prefix litera: <http://www.knora.org/ontology/0050/literature#>.
@prefix knora-base: <http://www.knora.org/ontology/knora-base#>.
@prefix salsah-gui: <http://www.knora.org/ontology/salsah-gui#>.

@base <http://www.knora.org/ontology/0059/text>.
@prefix text: <http://www.knora.org/ontology/0059/text#>.

<http://www.knora.org/ontology/0059/text>
	a owl:Ontology;
	dct:title "An ontology about text"@en;
	dct:description """Formal description of text in broadest sense, general subclasses, related classes, and properties."""@en;
	skos:note """Text editing is described in a seperate ontology"""@en;
	dct:creator "Hans Cools, MD, knowledge engineer, ontologist, software developer, NIE-INE, Basel University, Switzerland"@en;
	dct:contributor "Roberta Padlina, tool coordinator, NIE-INE, Basel University, Switzerland"@en;
	dct:publisher "Basel University, Switzerland"@en;
#	skos:note """Representation of an otherwise literal data element as object ('objectivation') enabling relating it to metadata"""@en.

	knora-base:attachedToProject <http://rdfh.ch/projects/0059>.

#
# CLASSES
#

text:Expression
	a owl:Class;
	rdfs:label "text expression"@en, "Text-Expression"@de;
	rdfs:comment """Expression as text in a human natural language."""@en;
	rdfs:subClassOf concept:Expression, language:HumanNaturalLanguageExpression, [
		a owl:Restriction; owl:onProperty text:hasAuthor; owl:minCardinality "0"^^xsd:nonNegativeInteger], [
		a owl:Restriction; owl:onProperty text:hasAuthorValue; owl:minCardinality "0"^^xsd:nonNegativeInteger], [
		a owl:Restriction; owl:onProperty text:hasRevisor; owl:minCardinality "0"^^xsd:nonNegativeInteger], [
		a owl:Restriction; owl:onProperty text:hasRevisorValue; owl:minCardinality "0"^^xsd:nonNegativeInteger], [
		a owl:Restriction; owl:onProperty text:hasCopyist; owl:minCardinality "0"^^xsd:nonNegativeInteger], [
		a owl:Restriction; owl:onProperty text:hasCopyistValue; owl:minCardinality "0"^^xsd:nonNegativeInteger], [
		a owl:Restriction; owl:onProperty text:hasIncipit; owl:minCardinality "0"^^xsd:nonNegativeInteger], [
		a owl:Restriction; owl:onProperty text:hasExplicit; owl:minCardinality "0"^^xsd:nonNegativeInteger], [
		a owl:Restriction; owl:onProperty text:hasVersionIndicator; owl:minCardinality "0"^^xsd:nonNegativeInteger], [
		a owl:Restriction; owl:onProperty text:hasReferenceText; owl:minCardinality "0"^^xsd:nonNegativeInteger], [
		a owl:Restriction; owl:onProperty text:hasReferenceTextValue; owl:minCardinality "0"^^xsd:nonNegativeInteger], [
		a owl:Restriction; owl:onProperty text-structure:hasStructure; owl:minCardinality "0"^^xsd:nonNegativeInteger], [
		a owl:Restriction; owl:onProperty text-structure:hasStructureValue; owl:minCardinality "0"^^xsd:nonNegativeInteger], [
		a owl:Restriction; owl:onProperty text-structure:hasWord; owl:minCardinality "0"^^xsd:nonNegativeInteger], [
		a owl:Restriction; owl:onProperty text-structure:hasWordValue; owl:minCardinality "0"^^xsd:nonNegativeInteger], [
		a owl:Restriction; owl:onProperty text-structure:hasSentence; owl:minCardinality "0"^^xsd:nonNegativeInteger], [
		a owl:Restriction; owl:onProperty text-structure:hasSentenceValue; owl:minCardinality "0"^^xsd:nonNegativeInteger], [
		a owl:Restriction; owl:onProperty text-structure:hasParagraph; owl:minCardinality "0"^^xsd:nonNegativeInteger], [
		a owl:Restriction; owl:onProperty text-structure:hasParagraphValue; owl:minCardinality "0"^^xsd:nonNegativeInteger], [
		a owl:Restriction; owl:onProperty text-structure:hasSection; owl:minCardinality "0"^^xsd:nonNegativeInteger], [
		a owl:Restriction; owl:onProperty text-structure:hasSectionValue; owl:minCardinality "0"^^xsd:nonNegativeInteger], [
		a owl:Restriction; owl:onProperty text-structure:hasProse; owl:minCardinality "0"^^xsd:nonNegativeInteger], [
		a owl:Restriction; owl:onProperty text-structure:hasProseValue; owl:minCardinality "0"^^xsd:nonNegativeInteger], [
		a owl:Restriction; owl:onProperty text-structure:hasLine; owl:minCardinality "0"^^xsd:nonNegativeInteger], [
		a owl:Restriction; owl:onProperty text-structure:hasLineValue; owl:minCardinality "0"^^xsd:nonNegativeInteger], [
		a owl:Restriction; owl:onProperty text-structure:hasLineNumber; owl:minCardinality "0"^^xsd:nonNegativeInteger], [
		a owl:Restriction; owl:onProperty text-structure:hasColumn; owl:minCardinality "0"^^xsd:nonNegativeInteger], [
		a owl:Restriction; owl:onProperty text-structure:hasColumnValue; owl:minCardinality "0"^^xsd:nonNegativeInteger], [
		a owl:Restriction; owl:onProperty text-structure:hasPage; owl:minCardinality "0"^^xsd:nonNegativeInteger], [
		a owl:Restriction; owl:onProperty text-structure:hasPageValue; owl:minCardinality "0"^^xsd:nonNegativeInteger], [
		a owl:Restriction; owl:onProperty textedit:hasEditor; owl:minCardinality "0"^^xsd:nonNegativeInteger], [
		a owl:Restriction; owl:onProperty textedit:hasEditorValue; owl:minCardinality "0"^^xsd:nonNegativeInteger], [
		a owl:Restriction; owl:onProperty textedit:hasGlossator; owl:minCardinality "0"^^xsd:nonNegativeInteger], [
		a owl:Restriction; owl:onProperty textedit:hasGlossatorValue; owl:minCardinality "0"^^xsd:nonNegativeInteger], [
		a owl:Restriction; owl:onProperty textedit:hasAbbreviator; owl:minCardinality "0"^^xsd:nonNegativeInteger], [
		a owl:Restriction; owl:onProperty textedit:hasAbbreviatorValue; owl:minCardinality "0"^^xsd:nonNegativeInteger], [
		a owl:Restriction; owl:onProperty textedit:hasRedactor; owl:minCardinality "0"^^xsd:nonNegativeInteger], [
		a owl:Restriction; owl:onProperty textedit:hasRedactorValue; owl:minCardinality "0"^^xsd:nonNegativeInteger], [
		a owl:Restriction; owl:onProperty textedit:hasEdition; owl:minCardinality "0"^^xsd:nonNegativeInteger], [
		a owl:Restriction; owl:onProperty textedit:hasEditionValue; owl:minCardinality "0"^^xsd:nonNegativeInteger], [
		a owl:Restriction; owl:onProperty textedit:hasSameEditionAs; owl:minCardinality "0"^^xsd:nonNegativeInteger], [
		a owl:Restriction; owl:onProperty textedit:hasSameEditionAsValue; owl:minCardinality "0"^^xsd:nonNegativeInteger], [
		a owl:Restriction; owl:onProperty textedit:hasDiplomaticTranscription; owl:minCardinality "0"^^xsd:nonNegativeInteger], [
		a owl:Restriction; owl:onProperty textedit:hasDiplomaticTranscriptionValue; owl:minCardinality "0"^^xsd:nonNegativeInteger], [
		a owl:Restriction; owl:onProperty textedit:hasCriticalEdition; owl:minCardinality "0"^^xsd:nonNegativeInteger], [
		a owl:Restriction; owl:onProperty textedit:hasCriticalEditionValue; owl:minCardinality "0"^^xsd:nonNegativeInteger].

text:Author
	a owl:Class;
	rdfs:label "author"@en, "Autor"@de;
	rdfs:comment """Role of a person being responsible for a text."""@en;
	skos:note """Often an author is also the creator of a text."""@en;
	rdfs:subClassOf human:Role.

text:Revisor
	a owl:Class;
	rdfs:label "revisor"@en, "Revisor"@de;
	rdfs:comment """Role of a person checking on certain aspects of a text."""@en;
	rdfs:subClassOf human:Role.

text:Copyist #* -> scholastic?
	a owl:Class;
	rdfs:label "scribes"@la, "copyist"@en, "Kopist"@de; # "scribe"@en, "Schreiber"@de;
	rdfs:comment """Role of a person copying text by handwriting."""@en;
	rdfs:subClassOf human:Creator.

text:Translator #* SC in scholastic: handwriting?
	a owl:Class;
	rdfs:label "translator"@en, "Ãœbersetzer"@de;
	rdfs:comment """Role of a person translating text by writing."""@en;
	rdfs:subClassOf language:PersonTranslator, human:Creator.

text:WrittenText
	a owl:Class;
	rdfs:label "written text"@en, "geschriebener Text"@de;
	rdfs:comment """Text written by any method, e.g. manually, with an analogue or digital typewriter, or on a computer, abstracted from its carrier."""@en;
	rdfs:subClassOf language:HumanNaturalLanguageExpression, [
		a owl:Restriction; owl:onProperty infocar:isWrittenWith; owl:minCardinality "0"^^xsd:nonNegativeInteger], [
		a owl:Restriction; owl:onProperty infocar:isWrittenWithValue; owl:minCardinality "0"^^xsd:nonNegativeInteger].

text:HandwrittenText
	a owl:Class;
	rdfs:label "handwritten text"@en, "handgeschriebener Text"@de;
	rdfs:comment """Text written by hand."""@en;
	rdfs:subClassOf text:WrittenText, [
		a owl:Restriction; owl:onProperty infocar:isInManuscript; owl:minCardinality "0"^^xsd:nonNegativeInteger], [
		a owl:Restriction; owl:onProperty infocar:isInManuscriptValue; owl:minCardinality "0"^^xsd:nonNegativeInteger].

text:TypewrittenText
	a owl:Class;
	rdfs:label "typewritten text"@en, "maschinengeschriebener Text"@de;
	rdfs:comment """Text written with a typewriter."""@en;
	rdfs:subClassOf text:WrittenText, [
		a owl:Restriction; owl:onProperty infocar:isInTypescript; owl:minCardinality "0"^^xsd:nonNegativeInteger], [
		a owl:Restriction; owl:onProperty infocar:isInTypescriptValue; owl:minCardinality "0"^^xsd:nonNegativeInteger]. #, [
#		a owl:Restriction; owl:onProperty infocar:isWrittenWith; owl:allValuesFrom text:Typewriter].

# text:Print: printed text abstracted from its carrier

text:DiaryEntry
	a owl:Class;
	rdfs:label "diary entry"@en, "Tagebucheintrag"@de;
	rdfs:comment """Periodical, usually daily description of a personal experience or observation written in a diary."""@en;
	rdfs:subClassOf text:Expression, [
		a owl:Restriction; owl:onProperty infocar:isInDiary; owl:minCardinality "0"^^xsd:nonNegativeInteger], [
		a owl:Restriction; owl:onProperty infocar:isInDiaryValue; owl:minCardinality "0"^^xsd:nonNegativeInteger], [
		a owl:Restriction; owl:onProperty infocar:hasDiaryEnteringDate; owl:minCardinality "0"^^xsd:nonNegativeInteger].

text:LetterExpression
	a owl:Class;
	rdfs:label "letter expression"@en, "Brief-Expression"@de;
	rdfs:comment """Text expression with a letter structure."""@en;
	rdfs:subClassOf text:Expression, [
#		a owl:Restriction; owl:onProperty text-structure:hasStructure; owl:allValuesFrom text-structure:LetterStructure], [
#		a owl:Restriction; owl:onProperty text-structure:hasStructure; owl:minCardinality "0"^^xsd:nonNegativeInteger], [
#		a owl:Restriction; owl:onProperty text-structure:hasStructureValue; owl:minCardinality "0"^^xsd:nonNegativeInteger], [
		a owl:Restriction; owl:onProperty infocar:isInLetter; owl:minCardinality "0"^^xsd:nonNegativeInteger], [
		a owl:Restriction; owl:onProperty infocar:isInLetterValue; owl:minCardinality "0"^^xsd:nonNegativeInteger].

text:Commentary
	a owl:Class;
	rdfs:label "commentary"@en, "Kommentar"@de;
	rdfs:comment """Text expression in the form of a series of comments as analysis, interpretation or explanation of something, especially another textual expression."""@en;
	rdfs:subClassOf text:Expression.

text:Draft
	a owl:Class;
	rdfs:label "draft"@en, "Entwurf"@de;
	rdfs:comment """Developmental text expression."""@en;
	rdfs:subClassOf human:CreationVersion.

#text:Transcription # homonym: from dif. expr. - eg. spoken - to written
#	a owl:Class;
#	rdfs:label "transcription"@en, "Transkription"@de;
#	rdfs:comment """Text expr copied by any method, e.g. handwriting, typewriting, machine copying, printing, digitizing."""@en;
#	rdfs:subClassOf language:HumanNaturalLanguageExpression.

text:Development
	a owl:Class;
	rdfs:label "text development"@en, "Text-Entwicklung"@de;
	rdfs:comment """Action wherein a person(s) creates text resulting in different manifestation, e.g. from notebook to manuscript to typescript to published print."""@en;
	rdfs:subClassOf human:Creating, [
		a owl:Restriction; owl:onProperty event:hasStage; owl:minCardinality "0"^^xsd:nonNegativeInteger], [
		a owl:Restriction; owl:onProperty event:hasStageValue; owl:minCardinality "0"^^xsd:nonNegativeInteger].

#* extrinsic feature: carrier, typescript, system of signs, diacritical eg. &
#* intrinsic: formal content

#*text:Witness
#	a owl:Class;
#	rdfs:label "witness"@en, "Textzeuge"@de;
#	rdfs:comment """Copy of an original text ."""@en; #* note: enabling its reconstruction, -> looking for features of originality
#	rdfs:subClassOf text:Transcription.

#
# PROPERTIES
#

text:hasText
	a owl:ObjectProperty;
	rdfs:label "has text"@en, "hat Text"@de;
	rdfs:comment """Relating a resource to a text (as object) as a writable coherent set of signs representing semantics in a language."""@en;
	rdfs:domain rdfs:Resource;
	rdfs:range rdfs:Literal;
	rdfs:subPropertyOf knora-base:hasValue;
	knora-base:subjectClassConstraint knora-base:Resource;
	knora-base:objectClassConstraint knora-base:TextValue;
	salsah-gui:guiElement salsah-gui:Richtext.

text:hasName
	a owl:ObjectProperty;
	rdfs:label "has name"@en, "hat Name"@de;
	rdfs:comment """Relating a resource to a name (as object) as a textual identifier of the resource."""@en;
	rdfs:subPropertyOf text:hasText; # rdfs:label, foaf:name
	knora-base:subjectClassConstraint knora-base:Resource;
	knora-base:objectClassConstraint knora-base:TextValue;
	salsah-gui:guiElement salsah-gui:Richtext.

text:hasPreferredName
	a owl:ObjectProperty;
	rdfs:label "has preferred name"@en, "hat bevorzugter Name"@de;
	rdfs:comment """Relating a resource to a preferred name (as object)."""@en;
	rdfs:subPropertyOf text:hasName;
	knora-base:subjectClassConstraint knora-base:Resource;
	knora-base:objectClassConstraint knora-base:TextValue;
	salsah-gui:guiElement salsah-gui:Richtext.

text:hasAlias
	a owl:ObjectProperty;
	rdfs:label "has alias"@en, "hat Alias"@de;
	rdfs:comment """Relating a resource to an alias (as object) as an alternative name of the resource."""@en;
	rdfs:subPropertyOf text:hasName;
	knora-base:subjectClassConstraint knora-base:Resource;
	knora-base:objectClassConstraint knora-base:TextValue;
	salsah-gui:guiElement salsah-gui:Richtext.

text:hasIdentifier # unique in context
	a owl:ObjectProperty;
	rdfs:label "has identifier"@en, "hat Kennzeichen"@de;
	rdfs:comment """Relating a resource to an identifier (as object) as a unique textual reference to the resource within a given context, and conforming to a formal identification system."""@en;
	rdfs:subPropertyOf text:hasText; #* P1_is_identified_by, domain: E1_CRM_Entity, range: E41_Appellation; cf. dcterms:identifier
	knora-base:subjectClassConstraint knora-base:Resource;
	knora-base:objectClassConstraint knora-base:TextValue;
	salsah-gui:guiElement salsah-gui:Richtext.

text:hasTitle
	a owl:ObjectProperty;
	rdfs:label "has title"@en, "hat Titel"@de;
	rdfs:comment """Relating a resource to a title as a textual identifier (as object) of the resource."""@en;
	rdfs:subPropertyOf text:hasText;
	knora-base:subjectClassConstraint knora-base:Resource;
	knora-base:objectClassConstraint knora-base:TextValue;
	salsah-gui:guiElement salsah-gui:Richtext.

text:hasComment
	a owl:ObjectProperty;
	rdfs:label "has comment"@en, "hat Kommentar"@de;
	rdfs:comment """Relating a resource to a comment (as object) as a textual statement about the resource."""@en;
	rdfs:subPropertyOf text:hasText;
	knora-base:subjectClassConstraint knora-base:Resource;
	knora-base:objectClassConstraint knora-base:TextValue;
	salsah-gui:guiElement salsah-gui:Richtext.

text:hasDescription
	a owl:ObjectProperty;
	rdfs:label "has description"@en, "hat Beschreibung"@de;
	rdfs:comment """Relating a resource to a description (as object) as a textual statement about features of the resource."""@en;
	rdfs:subPropertyOf text:hasText;
	knora-base:subjectClassConstraint knora-base:Resource;
	knora-base:objectClassConstraint knora-base:TextValue;
	salsah-gui:guiElement salsah-gui:Richtext.

text:hasDefinition
	a owl:ObjectProperty;
	rdfs:label "has definition"@en, "hat Definition"@de;
	rdfs:comment """Relating a resource to a definition (as object) as a textual statement about the essential features of the resource."""@en;
	rdfs:subPropertyOf text:hasDescription;
	knora-base:subjectClassConstraint knora-base:Resource;
	knora-base:objectClassConstraint knora-base:TextValue;
	salsah-gui:guiElement salsah-gui:Richtext.

text:hasDetailDescription
	a owl:ObjectProperty;
	rdfs:label "has detail description"@en, "hat Detail-Beschreibung"@de;
	rdfs:comment """Relating a resource to a description (as object) of its detail(s). E.g. in the case of a text a detail can be a passage variant or an emendation"""@en;
	rdfs:subPropertyOf text:hasDescription;
	knora-base:subjectClassConstraint knora-base:Resource;
	knora-base:objectClassConstraint knora-base:TextValue;
	salsah-gui:guiElement salsah-gui:Richtext.

text:hasSpecialDescription
	a owl:ObjectProperty;
	rdfs:label "has special description"@en, "hat Besonderes-Beschreibung"@de;
	rdfs:comment """Relating a resource to a description (as object) of (a) certain feature(s)."""@en;
	rdfs:subPropertyOf text:hasDescription;
	knora-base:subjectClassConstraint knora-base:Resource;
	knora-base:objectClassConstraint knora-base:TextValue;
	salsah-gui:guiElement salsah-gui:Richtext.

text:hasIncipit
	a owl:ObjectProperty;
	rdfs:label "has incipit"@en, "hat Incipit"@de;
	rdfs:comment """Relating an untitled text expression to a beginning part thereof (as object) to identify the text."""@en;
	rdfs:subPropertyOf text:hasText;
	knora-base:subjectClassConstraint text:Expression;
	knora-base:objectClassConstraint knora-base:TextValue;
	salsah-gui:guiElement salsah-gui:Richtext.

text:hasExplicit
	a owl:ObjectProperty;
	rdfs:label "has explicit"@en, "hat Explicit"@de;
	rdfs:comment """Relating an untitled text expression to an end part thereof (as object) to identify the text."""@en;
	rdfs:subPropertyOf text:hasText;
	knora-base:subjectClassConstraint text:Expression;
	knora-base:objectClassConstraint knora-base:TextValue;
	salsah-gui:guiElement salsah-gui:Richtext.

text:hasVersionIndicator
	a owl:ObjectProperty;
	rdfs:label "has version indicator"@en, "hat Version-Indikator"@de;
	rdfs:comment """Relating a text expression to a textual element (as object) that indicates its version."""@en;
	rdfs:subPropertyOf language:hasContent;
	knora-base:subjectClassConstraint text:Expression;
	knora-base:objectClassConstraint knora-base:TextValue;
	salsah-gui:guiElement salsah-gui:Richtext.

text:hasAuthor #*
	a owl:ObjectProperty;
	rdfs:label "has author"@en, "hat Autor"@de;
	rdfs:comment """Relating a text expression to a person who authored it."""@en;
	skos:note """A text can have more than one author."""@en;
	rdfs:domain text:Expression;
#	rdfs:range [rdfs:subClassOf human:Person, [a owl:Restriction; owl:onProperty human:hasRole; owl:someValuesFrom text:Author]];
	rdfs:subPropertyOf knora-base:hasLinkTo;
	knora-base:subjectClassConstraint text:Expression;
	knora-base:objectClassConstraint human:Person.

text:hasAuthorValue
	a owl:ObjectProperty;
	rdfs:label "has author - statement"@en, "hat Autor - Festlegung"@de;
	rdfs:comment """Relating a text expression to a reification statement of the relation between the text and a person who authored it."""@en;
	rdfs:subPropertyOf knora-base:hasLinkToValue;
	knora-base:subjectClassConstraint text:Expression;
	knora-base:objectClassConstraint knora-base:LinkValue.

#text:isAuthorOf
#	a owl:ObjectProperty;
#	rdfs:label "author of"@en;
#	rdfs:comment """Relating a person with author role to a text the person authored."""@en;
#	knora-base:subjectClassConstraint human:Person; # [rdfs:subClassOf human:Person, [a owl:Restriction; owl:onProperty human:hasRole; owl:someValuesFrom text:Author]];
#	knora-base:objectClassConstraint text:Expression.

text:hasRevisor
	a owl:ObjectProperty;
	rdfs:label "has revisor"@en, "hat Revisor"@de;
	rdfs:comment """Relating a text expression to a person who revised it."""@en;
	rdfs:domain text:Expression;
#	rdfs:range [rdfs:subClassOf human:Person, [a owl:Restriction; owl:onProperty human:hasRole; owl:someValuesFrom text:Revisor]];
	rdfs:subPropertyOf knora-base:hasLinkTo;
	knora-base:subjectClassConstraint text:Expression;
	knora-base:objectClassConstraint human:Person.

text:hasRevisorValue
	a owl:ObjectProperty;
	rdfs:label "has revisor - statement"@en, "hat Revisor - Festlegung"@de;
	rdfs:comment """Relating a text expression to a reification statement of the relation between the text and a person who revised it."""@en;
	rdfs:subPropertyOf knora-base:hasLinkToValue;
	knora-base:subjectClassConstraint text:Expression;
	knora-base:objectClassConstraint knora-base:LinkValue.

text:hasCopyist
	a owl:ObjectProperty;
	rdfs:label "has copyist"@en, "hat Kopist"@de;
	rdfs:comment """Relating a text to a person who copied it by handwriting."""@en;
	rdfs:domain text:Expression;
#	rdfs:range [rdfs:subClassOf human:Person, [a owl:Restriction; owl:onProperty human:hasRole; owl:someValuesFrom text:Copyist]];
	rdfs:subPropertyOf knora-base:hasLinkTo;
	knora-base:subjectClassConstraint text:Expression;
	knora-base:objectClassConstraint human:Person.

text:hasCopyistValue
	a owl:ObjectProperty;
	rdfs:label "has copyist - statement"@en, "hat Kopist - Festlegung"@de;
	rdfs:comment """Relating a text to a reification statement of the relation between the text and a person who copied it by handwriting."""@en;
	rdfs:subPropertyOf knora-base:hasLinkToValue;
	knora-base:subjectClassConstraint text:Expression;
	knora-base:objectClassConstraint knora-base:LinkValue.

text:hasReferenceText
	a owl:ObjectProperty;
	rdfs:label "has reference text"@en, "hat Bezugstext"@de;
	rdfs:comment "Relating a text to another one as its reference."@en;
	rdfs:subPropertyOf knora-base:hasLinkTo;
	knora-base:subjectClassConstraint text:Expression;
	knora-base:objectClassConstraint text:Expression.

text:hasReferenceTextValue
	a owl:ObjectProperty;
	rdfs:label "has reference text - statement"@en, "hat Bezugstext - Festlegung"@de;
	rdfs:comment "Relating a text to a reification statement of the relation between the text and another one as its reference."@en;
	rdfs:subPropertyOf knora-base:hasLinkToValue;
	knora-base:subjectClassConstraint text:Expression;
	knora-base:objectClassConstraint knora-base:LinkValue.